isolated refined fucntional program, sperated LE proof

sha/HMAC_proof.v
@@ -8,6 +8,7 @@ Local Open Scope logic.
 Require Import sha.spec_sha.
 
 Require Import sha.HMAC_functional_prog.
+Require Import sha.HMAC_refined_fp.
 
 Require Import sha.hmac_sha256.
 
@@ -15,11 +16,13 @@ Require Import HMAC_definitions.
 (*Require Import HMAC_part2LE. this file contains the implementation for the path key_len <= 64*)
 (*Require Import HMAC_part2GT. this file contains the implementation for the path key_len > 64*)
 
-Declare Module PART2LE: HMAC_PART2LE.
+(*Declare Module PART2LE: HMAC_PART2LE.*)
 Declare Module PART2GT: HMAC_PART2GT.
 
-Definition restLE := PART2LE.HMAC_LE.
+(*Definition restLE := PART2LE.HMAC_LE.*)
 Definition restGT := PART2GT.HMAC_GT.
+
+Require Import HMAC_LoopBodyGT.
 
 Lemma body_hmac_sha256: semax_body Vprog Gtot 
       f_hmac_sha256 hmac_spec.
@@ -102,7 +105,7 @@ forward_if (ASSN_SuperCanon topshares argshares A ANEW KV
         rewrite int_max_signed_eq. omega.
       entailer. unfold repr_key.
       apply derives_trans with (Q:=!!(isptr (KEY A) /\ Forall isbyteZ (key a))).
-           entailer. abstract normalize.
+           entailer. normalize. split; trivial. rewrite int_max_unsigned_eq. rewrite int_max_signed_eq in HA1a. omega.
     rewrite <- AxiomK. cancel.
       rewrite memory_block_array_tuchar; try omega.
       rewrite memory_block_array_tuchar; try omega.
@@ -201,6 +204,7 @@ destruct KLENGTH.
      simpl. rewrite <- HeqKLENGTH. simpl. reflexivity.
   unfold repr_key_len, repr_text_len in H1. rewrite TN, KN, TLN, KLN in H1.
   clear H1. (*all conjuncts are trivial, or equal to assumptions we already have*)
+  clear H0.
 
   assert (TLrange: 0 <= text_len a <= Int.max_unsigned).
     clear - HH3. destruct HH3.
@@ -215,6 +219,7 @@ destruct KLENGTH.
   assert (TKN: tk (locals h1) = functional_prog.SHA_256' (key a)).
      rewrite Heqh1, Heqh0. unfold HMAC_Refined.snippet1. simpl.
      rewrite <- HeqKLENGTH. simpl. reflexivity.
+
   forward_call (* memset *) (Tsh, k_ipad VALS, 65, Int.zero).
   { assert (FR: Frame = [
         `(data_at_ Tsh (tarray tuchar 65) (k_opad VALS)),
@@ -232,13 +237,14 @@ destruct KLENGTH.
     rewrite TKN.
     entailer.
     apply andp_right.
-      rewrite <- H6; clear H6. simpl.
+      rewrite <- H5; clear H5. simpl.
       rewrite (data_at__isptr _ _ (k_ipad VALS)). abstract entailer.
     assert (SF: Int.repr 65 = Int.repr (sizeof (tarray tuchar 65))) by reflexivity.
     rewrite SF, align_1_memory_block_data_at_; trivial.
    }
    after_call. 
    (*Warning: Collision between bound variables of name x *)
+   subst retval0.
 
   forward_call (* memset *) (Tsh, k_opad VALS, 65, Int.zero).
   { assert (FR: Frame = [
@@ -257,14 +263,14 @@ destruct KLENGTH.
     entailer.
     rewrite TKN.
     apply andp_right.
-      rewrite <- H7; clear H7. simpl.
+      rewrite <- H6; clear H6. simpl.
       rewrite (data_at__isptr _ _ (k_opad VALS)). abstract entailer.
     assert (SF: Int.repr 65 = Int.repr (sizeof (tarray tuchar 65))) by reflexivity.
     rewrite SF, align_1_memory_block_data_at_; trivial. cancel.
    }
    after_call. 
    (*Warning: Collision between bound variables of name x *) 
-   subst retval1.
+   subst retval0.
 
    assert (ZLenSha: Zlength (tk (locals h1)) = 32).
      rewrite TKN, Zlength_correct.
@@ -299,7 +305,7 @@ destruct KLENGTH.
    `(memory_block dsh (Int.repr 32) (DIGEST A))))).
    abstract entailer.
 
-   normalize. rename H1 into isByteKey. rename H2 into isByteShaKey.
+   normalize. rename H into isByteKey. rename H0 into isByteShaKey.
 
    (* following this recipe doesn't quite work, since some rewrite rule is missing to cleanup
       the postcondition after after_call
@@ -340,7 +346,7 @@ destruct KLENGTH.
    after_call. 
    (*Warning: Collision between bound variables of name x *)
    subst WITNESS. normalize. 
-   subst retval1. 
+   subst retval0. 
 
    (**************** memcpy( k_opad, key, key_len ) ******)
 (*   frame_SEP does not apply for some reason*)
@@ -375,14 +381,14 @@ destruct KLENGTH.
    } 
    after_call. 
    subst WITNESS. normalize. 
-   subst retval0 retval1. 
+   subst retval0. 
 
    (***************for -loop*********************)
      rewrite (split_array_at 64 tuchar Tsh _ 32 65); try omega.
      rewrite (split_array_at 64 tuchar Tsh _ 32 65); try omega.
   normalize.
   eapply semax_seq'. 
-  frame_SEP 0 2 5 6. (*different numbers than in ELSE - but what we want is all terms for k_ipad, k_opad below index 64*)
+  frame_SEP 5 0 6 2. (* we want iall terms for k_ipad, k_opad below index 64*)
   unfold isbyteZ in isByteShaKey. 
   forward_for_simple_bound 64 (EX i:Z, 
   (PROP  ()
@@ -404,11 +410,7 @@ destruct KLENGTH.
        i 64 (k_opad VALS));
    `(array_at tuchar Tsh
        (cVint (force_int oo ZnthV tuchar (map Vint (map Int.repr (map Byte.unsigned (map Byte.repr (HMAC_FUN.mkKey (key a))))))))
-       i 64 (k_ipad VALS));(*
-   `(array_at tuchar Tsh (fun _ : Z => Vint Int.zero)
-       64 65(k_opad VALS));
-   `(array_at tuchar Tsh (fun _ : Z => Vint Int.zero)
-       64 65 (k_ipad VALS));*)
+       i 64 (k_ipad VALS));
    `(array_at tuchar Tsh
        (cVint (force_int oo ZnthV tuchar (map Vint (map Int.repr (map Byte.unsigned (HMAC_FUN.mkArg (map Byte.repr (HMAC_FUN.mkKey (key a))) Opad))))))
        0 i (k_opad VALS));
@@ -431,29 +433,30 @@ destruct KLENGTH.
      { intros; unfold cVint. f_equal; simpl.
        unfold ZnthV. destruct (zlt i 0); simpl; trivial.
        assert (I: (0 <= Z.to_nat i < length (functional_prog.SHA_256' (key a)))%nat).
-          clear - H9. destruct H9. split; try omega.
+          clear - H8. destruct H8. split; try omega.
           rewrite length_SHA256'. simpl. apply Z2Nat.inj_lt in H0. apply H0.
           trivial. omega.
        unfold HMAC_FUN.mkKey. simpl. rewrite HH9, <- HeqKLENGTH.
        unfold HMAC_FUN.zeroPad. rewrite map_app.  rewrite map_app.  rewrite map_app.  
        destruct (nth_mapVint (Z.to_nat i) (functional_prog.SHA_256' (key a))); trivial.
-       rewrite H10. (* simpl. rewrite map_map. rewrite map_map.*)
+       rewrite H9. (* simpl. rewrite map_map. rewrite map_map.*)
        rewrite app_nth1.
        2: repeat rewrite map_length; apply I.  
-       rewrite <- nth_default_eq in H10. unfold nth_default in H10.
+       rewrite <- nth_default_eq in H9. unfold nth_default in H9.
        remember (nth_error
           (map Vint (map Int.repr (functional_prog.SHA_256' (key a))))
           (Z.to_nat i)) as d. 
-       destruct d; inversion H10. clear H10; subst v. 
+       destruct d; inversion H9. clear H9; subst v. 
        apply eq_sym in Heqd. destruct (map_nth_error_inv _ _ _  _ Heqd) as [? [? ?]].
-       inv H11; clear Heqd. destruct (map_nth_error_inv _ _ _  _ H10) as [? [? ?]]. subst x0; clear H10.
+       inv H10; clear Heqd. destruct (map_nth_error_inv _ _ _  _ H9) as [? [? ?]]. 
+       subst x0; clear H9.
        rewrite nth_map' with (d':=Int.zero). 
        rewrite nth_map' with (d':=Byte.repr Z0). 
        rewrite nth_map' with (d':=Z0). 
-       rewrite <- nth_default_eq. unfold nth_default. rewrite H11.
+       rewrite <- nth_default_eq. unfold nth_default. rewrite H10.
        rewrite Byte.unsigned_repr. trivial.
        rewrite Forall_forall in isByteShaKey. 
-       apply nth_error_in in H11. apply isByteShaKey in H11.
+       apply nth_error_in in H10. apply isByteShaKey in H10.
          unfold Byte.max_unsigned, Byte.modulus, Byte.wordsize. simpl. omega.
        apply I.
        rewrite map_length. apply I.
@@ -466,15 +469,15 @@ destruct KLENGTH.
            (map (fun x : byte => Int.repr (Byte.unsigned x))
               (map Byte.repr (HMAC_FUN.mkKey (key a)))))) i).
      { unfold cVint; simpl. intros. f_equal. 
-       unfold ZnthV. if_tac. omega. clear H10. 
+       unfold ZnthV. if_tac. omega. clear H9. 
        assert (L: (Z.to_nat i < length (HMAC_FUN.mkKey (key a)))%nat).
-          clear - H9. destruct H9. rewrite HMAC_FUN.mkKey_length. unfold SHA256_BlockSize.
+          clear - H8. destruct H8. rewrite HMAC_FUN.mkKey_length. unfold SHA256_BlockSize.
           apply Z2Nat.inj_lt in H0. simpl in H0. omega. omega. omega.
        rewrite nth_map' with (d':=Int.zero).
          rewrite nth_map' with (d':=Byte.repr Z0). 
            rewrite nth_map' with (d':=Z0).
              unfold HMAC_FUN.mkKey. simpl. rewrite HH9, <- HeqKLENGTH.
-             unfold HMAC_FUN.zeroPad. clear - H9. destruct H9 as [X Y]. 
+             unfold HMAC_FUN.zeroPad. clear - H8. destruct H8 as [X Y]. 
              rewrite app_nth2.
                rewrite nth_Nlist. reflexivity.   
                rewrite length_SHA256'. simpl.
@@ -489,266 +492,12 @@ destruct KLENGTH.
      rewrite <- (array_at_ext tuchar Tsh _ _ _ _ EQ2). abstract cancel.
    }
    { (*show that body satisfies "invariant"*)
-     admit. (*Require Import HMAC_LoopBodyGT.
-     eapply (loopbody Espec tsh ksh dsh); try eassumption.*)
+     eapply (loopbodyGT Espec); try eassumption.
    }    
    { (*show increment*) trivial. (*normalize.*) }
    unfold update_tycon; simpl.
-   repeat rewrite array_at_emp; simpl. normalize. (*WHY are the two `emp terms not eliminated here???*)
+   repeat rewrite array_at_emp; simpl. normalize. 
 
-(****************** continuation after for-loop **************************)
-(*   (***************for -loop*********************)
-  eapply semax_seq'. 
-  frame_SEP 1 2 3 4. (*different numbers than in ELSE - but what we want is all terms for k_ipad, k_opad*)
-  unfold isbyteZ in isByteShaKey. 
-  forward_for_simple_bound 64 (EX i:Z, 
-  (PROP  ()
-   LOCAL  (`(eq (TEXT A)) (eval_id _text); `(eq (tk VALS)) (eval_id _key);
-   `(eq KV0) (eval_var sha._K256 (tarray tuint 64));
-   `(eq (Vint (Int.repr (text_len a)))) (eval_id _text_len);
-   `(eq (Vint (Int.repr 32))) (eval_id _key_len);
-   `(eq (DIGEST A)) (eval_id _digest);
-   `(eq (k_ipad VALS)) (eval_var _k_ipad (tarray tuchar 65));
-   `(eq (k_opad VALS)) (eval_var _k_opad (tarray tuchar 65));
-   `(eq (tk VALS)) (eval_var _tk (tarray tuchar 32));
-   `(eq (tk2 VALS)) (eval_var _tk2 (tarray tuchar 32));
-   `(eq (bufferIn VALS)) (eval_var _bufferIn (tarray tuchar 1024));
-   `(eq (bufferOut VALS)) (eval_var _bufferOut (tarray tuchar 1024)))
-   SEP 
-   (
-   `(array_at tuchar Tsh
-       (cVint (force_int oo ZnthV tuchar (map Vint (map Int.repr (map Byte.unsigned (map Byte.repr (HMAC_FUN.mkKey (key a))))))))
-       i 64 (k_opad VALS));
-   `(array_at tuchar Tsh
-       (cVint (force_int oo ZnthV tuchar (map Vint (map Int.repr (map Byte.unsigned (map Byte.repr (HMAC_FUN.mkKey (key a))))))))
-       i 64 (k_ipad VALS));
-   `(array_at tuchar Tsh (fun _ : Z => Vint Int.zero)
-       64 65(k_opad VALS));
-   `(array_at tuchar Tsh (fun _ : Z => Vint Int.zero)
-       64 65 (k_ipad VALS));
-   `(array_at tuchar Tsh
-       (cVint (force_int oo ZnthV tuchar (map Vint (map Int.repr (map Byte.unsigned (HMAC_FUN.mkArg (map Byte.repr (HMAC_FUN.mkKey (key a))) Opad))))))
-       0 i (k_opad VALS));
-   `(array_at tuchar Tsh
-       (cVint (force_int oo ZnthV tuchar (map Vint (map Int.repr (map Byte.unsigned (HMAC_FUN.mkArg (map Byte.repr (HMAC_FUN.mkKey (key a))) Ipad))))))
-       0 i (k_ipad VALS))))).
-   
-   { (*precondition implies "invariant"*)
-     entailer. rewrite array_at_emp. rewrite array_at_emp. entailer.
-     apply andp_right. entailer. unfold array_at. entailer.
-     repeat rewrite (map_map Byte.unsigned). 
-     rewrite (split_array_at 64 tuchar Tsh _ 32 65); try omega.
-     rewrite (split_array_at 64 tuchar Tsh _ 32 65); try omega.
-     cancel.
-     rewrite (split_array_at 32 tuchar Tsh _ 0 64); try omega.
-     rewrite (split_array_at 32 tuchar Tsh _ 0 64); try omega.
-     assert (EQ: forall i, 0 <= i < 32 ->
-         cVint (force_int oo ZnthV tuchar
-            (map Vint (map Int.repr (functional_prog.SHA_256' (key a))))) i =
-        cVint (force_int oo ZnthV tuchar
-           (map Vint (map (fun x : byte => Int.repr (Byte.unsigned x))
-                   (map Byte.repr (HMAC_FUN.mkKey (key a)))))) i).
-     { intros; unfold cVint. f_equal; simpl.
-       unfold ZnthV. destruct (zlt i 0); simpl; trivial.
-       assert (I: (0 <= Z.to_nat i < length (functional_prog.SHA_256' (key a)))%nat).
-          clear - H9. destruct H9. split; try omega.
-          rewrite length_SHA256'. simpl. apply Z2Nat.inj_lt in H0. apply H0.
-          trivial. omega.
-       unfold HMAC_FUN.mkKey. simpl. rewrite HH9, <- HeqKLENGTH.
-       unfold HMAC_FUN.zeroPad. rewrite map_app.  rewrite map_app.  rewrite map_app.  
-       destruct (nth_mapVint (Z.to_nat i) (functional_prog.SHA_256' (key a))); trivial.
-       rewrite H10. (* simpl. rewrite map_map. rewrite map_map.*)
-       rewrite app_nth1.
-       Focus 2. repeat rewrite map_length. apply I. 
-       rewrite <- nth_default_eq in H10. unfold nth_default in H10.
-       remember (nth_error
-          (map Vint (map Int.repr (functional_prog.SHA_256' (key a))))
-          (Z.to_nat i)) as d. 
-       destruct d; inversion H10. clear H10; subst v. 
-       apply eq_sym in Heqd. destruct (map_nth_error_inv _ _ _  _ Heqd) as [? [? ?]].
-       inv H11; clear Heqd. destruct (map_nth_error_inv _ _ _  _ H10) as [? [? ?]]. subst x0; clear H10.
-       rewrite nth_map' with (d':=Int.zero). 
-       rewrite nth_map' with (d':=Byte.repr Z0). 
-       rewrite nth_map' with (d':=Z0). 
-       rewrite <- nth_default_eq. unfold nth_default. rewrite H11.
-       rewrite Byte.unsigned_repr. trivial.
-       rewrite Forall_forall in isByteShaKey. 
-       apply nth_error_in in H11. apply isByteShaKey in H11.
-         unfold Byte.max_unsigned, Byte.modulus, Byte.wordsize. simpl. omega.
-       apply I.
-       rewrite map_length. apply I.
-       repeat rewrite map_length. apply I.
-     }
-     assert (EQ2: forall i : Z, 32 <= i < 64 ->
-        Vint Int.zero =
-        cVint (force_int oo ZnthV tuchar
-         (map Vint
-           (map (fun x : byte => Int.repr (Byte.unsigned x))
-              (map Byte.repr (HMAC_FUN.mkKey (key a)))))) i).
-     { unfold cVint; simpl. intros. f_equal. 
-       unfold ZnthV. if_tac. omega. clear H10. 
-       assert (L: (Z.to_nat i < length (HMAC_FUN.mkKey (key a)))%nat).
-          clear - H9. destruct H9. rewrite HMAC_FUN.mkKey_length. unfold SHA256_BlockSize.
-          apply Z2Nat.inj_lt in H0. simpl in H0. omega. omega. omega.
-       rewrite nth_map' with (d':=Int.zero).
-       Focus 2. repeat rewrite map_length. apply L.
-       rewrite nth_map' with (d':=Byte.repr Z0). 
-       Focus 2. repeat rewrite map_length. apply L.
-       rewrite nth_map' with (d':=Z0).
-       Focus 2. repeat rewrite map_length. apply L. 
-       unfold HMAC_FUN.mkKey. simpl. rewrite HH9, <- HeqKLENGTH.
-          unfold HMAC_FUN.zeroPad. rewrite app_nth2.
-          Focus 2. clear - H9. destruct H9. rewrite length_SHA256'. simpl.
-                   apply Z2Nat.inj_le in H. simpl in H. omega. omega. omega.
-          rewrite nth_Nlist. reflexivity. 
-          clear - H9. destruct H9. rewrite length_SHA256'. simpl.
-                   apply Z2Nat.inj_lt in H0. simpl in H0. omega. omega. omega. 
-     }
-     repeat rewrite sepcon_assoc.
-     apply sepcon_derives. apply array_at_ext'; assumption. 
-     apply sepcon_derives. apply array_at_ext'; assumption. 
-     apply sepcon_derives. apply array_at_ext'; assumption. 
-                           apply array_at_ext'; assumption. 
-   }
-   { (*show that body satisfies "invariant"*)
-     Require Import HMAC_LoopBodyGT.
-     remember (cVint
-             (force_int
-              oo ZnthV tuchar
-                   (map Vint
-                      (map Int.repr
-                         (map Byte.unsigned
-                            (map Byte.repr (HMAC_FUN.mkKey (key a)))))))) as KKEY.
-     remember (cVint
-            (force_int
-             oo ZnthV tuchar
-                  (map Vint
-                     (map Int.repr
-                        (map Byte.unsigned
-                           (HMAC_FUN.mkArg
-                              (map Byte.repr (HMAC_FUN.mkKey (key a))) Opad)))))) as OPAD.
-     remember (cVint
-            (force_int
-             oo ZnthV tuchar
-                  (map Vint
-                     (map Int.repr
-                        (map Byte.unsigned
-                           (HMAC_FUN.mkArg
-                              (map Byte.repr (HMAC_FUN.mkKey (key a))) Ipad)))))) as IPAD.
-     eapply (loopbody Espec tsh ksh dsh); try eassumption.
-(*
-unfold MORE_COMMANDS, POSTCONDITION, abbreviate.
-     remember (cVint
-             (force_int
-              oo ZnthV tuchar
-                   (map Vint
-                      (map Int.repr
-                         (map Byte.unsigned
-                            (map Byte.repr (HMAC_FUN.mkKey (key a)))))))) as KKEY.
-     remember (cVint
-            (force_int
-             oo ZnthV tuchar
-                  (map Vint
-                     (map Int.repr
-                        (map Byte.unsigned
-                           (HMAC_FUN.mkArg
-                              (map Byte.repr (HMAC_FUN.mkKey (key a))) Opad)))))) as OPAD.
-     remember (cVint
-            (force_int
-             oo ZnthV tuchar
-                  (map Vint
-                     (map Int.repr
-                        (map Byte.unsigned
-                           (HMAC_FUN.mkArg
-                              (map Byte.repr (HMAC_FUN.mkKey (key a))) Ipad)))))) as IPAD.
-     simple eapply semax_seq'.
-
-eapply semax_pre0; [ apply now_later | ].
-eapply semax_post_flipped'.
-   eapply NEWsemax_loadstore_array. 
-     reflexivity. trivial. reflexivity. reflexivity.  reflexivity.
-
-rewrite (array_at_isptr tuchar _ _ _ 64 (k_ipad VALS)).
-rewrite (array_at_isptr tuchar _ _ _ 64 (k_opad VALS)).
-  go_lowerx. normalize.
-  repeat instantiate_Vptr; repeat apply andp_right.
-     instantiate (1:=k_ipad VALS). 
-      destruct (k_ipad VALS); try contradiction. rewrite H10. clear - H10.
-       unfold eval_var in H10. remember (Map.get (ve_of rho) _k_ipad) as d. destruct d.
-         destruct p. remember (eqb_type (tarray tuchar 65) t) as bb.
-         destruct bb; inv H10; apply eq_sym in Heqbb.
-         apply eqb_type_spec in Heqbb. subst t. apply eq_sym in Heqd.  rel_expr. instantiate (1:=b0). entailer.
-         simpl. instantiate (1:=Tsh).
-         rewrite (split3_array_at' i tuchar Tsh _ i _ (eval_var _k_ipad (tarray tuchar 65) rho) (eval_var _k_ipad (tarray tuchar 65) rho)).
-         unfold add_ptr_int; simpl. Focus 2. admit. 
-  destruct (k_opad VALS); try contradiction.
-  repeat instantiate_Vptr; repeat apply andp_right.
-     instantiate (1:=k_ipad VALS). rewrite H10. clear - H10. unfold eval_var in H10. rel_expr. repeat instantiate_Vptr; repeat apply andp_right.
-  rel_expr. rel_expr. admit.array_at_local_facts
-                        instantiate (1:=i). rel_expr. admit.
-     Focus 5. simpl. reflexivity. Locate semax_loadstore_array'. 2: reflexivity. 2: trivial. 2: reflexivity.
-     Focus 4. apply andp_right.  
-                apply andp_right.
-
-SearchAbout rel_lvalue. rel_expr.
-          instantiate (1:= i). instantiate (1:= k_ipad VALS). rel_expr.
-eauto.
-                  apply rel_expr_array_load. reflexivity 
-     hoist_later_in_pre.
-     simple eapply semax_seq'.
-   eapply semax_loadstore_array.
-   simple eapply (semax_loadstore_array sx);
-      remember (Ederef
-        (Ebinop Oadd (Evar _k_ipad (tarray tuchar 65)) (Etempvar _i tint)
-           (tptr tuchar)) tuchar) as e1.
-        eapply semax_loadstore_array'.
-assert (typeof e1 = tuchar). subst e1. simpl. reflexivity.
-      remember (Ederef
-        (Ebinop Oadd (Evar _k_ipad (tptr tuchar)) (Etempvar _i tint)
-           (tptr tuchar)) tuchar) as e1'.
-assert (typeof e1' = tuchar). subst e1'. simpl. reflexivity.
-          reflexivity. apply I. reflexivity.
-        Focus 8. entailer. 
-          repeat apply andp_right. 
-         (*rel_expr (Evar _k_ipad (tarray tuchar 65)) ?7539 rho*)
-          Focus 2. eapply rel_expr_cast.
-                   eapply rel_expr_binop.
-          instantiate (1:= k_ipad VALS). rel_expr. unfold eval_var in H7.
-          Focus 2. rel_expr.
-          Focus 2. eapply rel_expr_cast.
-                   eapply rel_expr_binop. 
-                   (* rel_expr
-(*        eapply semax_loadstore_array.?*)
-          reflexivity. apply I. reflexivity. admit. (*TODO tarray/tptr*)
-          reflexivity. 
-        entailer. 
-          repeat apply andp_right. 
-         (*rel_expr (Evar _k_ipad (tarray tuchar 65)) ?7539 rho*)
-          instantiate (1:= k_ipad VALS). rel_expr. unfold eval_var in H7.
-          Focus 2. rel_expr.
-          Focus 2. eapply rel_expr_cast.
-                   eapply rel_expr_binop. 
-                   (* rel_expr
-      (Ederef
-         (Ebinop *)
-                  Focus 2. rel_expr. 
-                  Focus 2. simpl. eapply rel_expr_deref.
-                  rel_expr. auto.
-                apply andp_right. 
-SearchAbout rel_lvalue. rel_expr. 
-           eapply rel_expr_array_load'.
-       reflexivity. apply I. reflexivity.
-     simple eapply semax_loadstore_array.
-       reflexivity. apply I. reflexivity.
-       unfold tarray; simpl. admit. (*TODO: refine Lemma semax_loadstore_array' in array_lemmas.v*)
-       reflexivity.
-     *)*)
-   }
-    
-   { (*show increment*) normalize. }
-   normalize. unfold update_tycon; simpl.
-   repeat rewrite array_at_emp; simpl. normalize. (*WHY are the two `emp terms not eliminated here???*)
-*)
 (****************** continuation after for-loop **************************)
  remember (map Byte.unsigned
                          (HMAC_FUN.mkArg
@@ -766,464 +515,14 @@ SearchAbout rel_lvalue. rel_expr.
                 (map Vint (map Int.repr KOPAD))) as OPAD.
   remember (force_int oo ZnthV tuchar (map Vint (map Int.repr (functional_prog.SHA_256' (key a))))) as KKEY. 
  remember (fun _ : Z => Vint Int.zero) as ZERO.
+rewrite Zplus_comm in TL1024. 
+
 eapply semax_pre0.
-Focus 2. rewrite Zplus_comm in TL1024. solve [eapply restGT; eassumption].
+2: solve [eapply restGT; eassumption].
 abstract solve [entailer; cancel].
 }
 
 { (* case key_len a <= 64 *) 
-  unfold HMAC_Refined.snippet1; simpl.
-  remember (HMAC_Refined.initLocalVals).
-  subst ANEW. 
-  assert (Heq: h1 = h0). 
-    subst h1. subst h0. 
-         unfold HMAC_Refined.snippet1; simpl.
-         rewrite <- HeqKLENGTH. reflexivity.
-  clear Heqh1. subst h1. clear H1 Heqanew anew.
-  subst argshares.
-  destruct H as [[HH1 HH2] [[HH3 [HH4 TL1024]] [HH5 [HH6 [HH7 [HH8 HH9]]]]]].
-  rewrite HH4 in *.
-  assert (TLrange: 0 <= text_len a <= Int.max_unsigned).
-    clear - HH3. destruct HH3.
-    rewrite int_max_signed_eq in H0. rewrite int_max_unsigned_eq. omega.
-  simpl in HH8. rewrite Int.unsigned_repr in HH8; trivial.
-  assert (KLrange: 0 <= key_len a <= Int.max_unsigned).
-    clear - HH1. destruct HH1.
-    rewrite int_max_signed_eq in H0. rewrite int_max_unsigned_eq. omega.
-  rewrite HH2 in HH9; simpl in HH9.
-    rewrite Int.unsigned_repr in HH9; trivial.
-
-
-  forward_call (* memset *) (Tsh, k_ipad VALS, 65, Int.zero).
-  { assert (FR: Frame = [
-        `(data_at_ Tsh (tarray tuchar 65) (k_opad VALS)),
-        `(data_at_ Tsh (tarray tuchar 32) (tk VALS)),
-        `(data_at_ Tsh (tarray tuchar 32) (tk2 VALS)),
-        `(data_at_ Tsh (tarray tuchar 1024) (bufferIn VALS)),
-        `(data_at_ Tsh (tarray tuchar 1024) (bufferOut VALS)), 
-        `(K_vector KV),
-        `(repr_key a ksh (KEY A)),
-        `(repr_text a tsh (TEXT A)),
-        `(memory_block dsh (Int.repr 32) (DIGEST A))]).  
-      subst Frame. reflexivity. 
-    rewrite FR. clear FR Frame.
-    unfold repr_locals; simpl. intros rho.
-    entailer.
-    apply andp_right.
-      rewrite <- H6; clear H6. simpl.
-      rewrite (data_at__isptr _ _ (k_ipad VALS)). abstract entailer.
-    assert (SF: Int.repr 65 = Int.repr (sizeof (tarray tuchar 65))) by reflexivity.
-    rewrite SF, align_1_memory_block_data_at_; trivial.
-   }
-   after_call. 
-   (*Warning: Collision between bound variables of name x *)
-
-  forward_call (* memset *) (Tsh, k_opad VALS, 65, Int.zero).
-  { assert (FR: Frame = [
-        `(array_at tuchar Tsh (fun _ : Z => Vint Int.zero) 0 65 (k_ipad VALS)),
-        `(data_at_ Tsh (tarray tuchar 32) (tk VALS)),
-        `(data_at_ Tsh (tarray tuchar 32) (tk2 VALS)),
-        `(data_at_ Tsh (tarray tuchar 1024) (bufferIn VALS)),
-        `(data_at_ Tsh (tarray tuchar 1024) (bufferOut VALS)), 
-        `(K_vector KV),
-        `(repr_key a ksh (KEY A)),
-        `(repr_text a tsh (TEXT A)),
-        `(memory_block dsh (Int.repr 32) (DIGEST A))]).  
-      subst Frame. reflexivity.
-    rewrite FR. clear FR Frame.
-    unfold repr_locals; simpl. intros rho.
-    entailer.
-    apply andp_right.
-      rewrite <- H7; clear H7. simpl.
-      rewrite (data_at__isptr _ _ (k_opad VALS)). abstract entailer.
-    assert (SF: Int.repr 65 = Int.repr (sizeof (tarray tuchar 65))) by reflexivity.
-    rewrite SF, align_1_memory_block_data_at_; trivial. abstract cancel.
-   }
-   after_call. 
-   (*Warning: Collision between bound variables of name x *) 
-   subst retval1.
-
-   (**************** memcpy( k_ipad, key, key_len ) ******)
-   unfold repr_key, data_block. 
-   eapply semax_pre with (P' :=(PROP (Forall isbyteZ (key a))
-   LOCAL  (
-   `(eq (TEXT A)) (eval_id _text); `(eq (KEY A)) (eval_id _key);
-   `(eq KV) (eval_var sha._K256 (tarray tuint 64));
-   `(eq (TEXTLEN A)) (eval_id _text_len);
-   `(eq (KEYLEN A)) (eval_id _key_len); `(eq (DIGEST A)) (eval_id _digest);
-   `(eq (k_ipad VALS)) (eval_var _k_ipad (tarray tuchar 65));
-   `(eq (k_opad VALS)) (eval_var _k_opad (tarray tuchar 65));
-   `(eq (tk VALS)) (eval_var _tk (tarray tuchar 32));
-   `(eq (tk2 VALS)) (eval_var _tk2 (tarray tuchar 32));
-   `(eq (bufferIn VALS)) (eval_var _bufferIn (tarray tuchar 1024));
-   `(eq (bufferOut VALS)) (eval_var _bufferOut (tarray tuchar 1024)))
-   SEP 
-   (`(array_at tuchar Tsh (fun _ : Z => Vint Int.zero) 0 65 (k_opad VALS));
-   `(array_at tuchar Tsh (fun _ : Z => Vint Int.zero) 0 65 (k_ipad VALS));
-   `(data_at_ Tsh (tarray tuchar 32) (tk VALS));
-   `(data_at_ Tsh (tarray tuchar 32) (tk2 VALS));
-   `(data_at_ Tsh (tarray tuchar 1024) (bufferIn VALS));
-   `(data_at_ Tsh (tarray tuchar 1024) (bufferOut VALS)); `(K_vector KV);
-   `(array_at tuchar ksh (tuchars (map Int.repr (key a))) 0 (Zlength (key a))
-       (KEY A)); `(repr_text a tsh (TEXT A));
-   `(memory_block dsh (Int.repr 32) (DIGEST A))))).
-     abstract entailer. 
-
-   normalize. rename H1 into isByteKey.
-
-   (* following this recipe doesn't quite work, since some rewrite rule is missing to cleanup
-      the postcondition after after_call
-   eapply semax_seq'.
-   frame_SEP 7 1.*)
-   remember (ksh, Tsh, k_ipad VALS, KEY A, key_len a, 
-            force_int oo (ZnthV tuchar (map Vint (map Int.repr (key a))))
-       ) as WITNESS. 
-   forward_call (* memcopy *) WITNESS.
-   { rewrite HeqWITNESS; clear HeqWITNESS WITNESS.
-     assert (FR: Frame =
-       [`(array_at tuchar Tsh (fun _ : Z => Vint Int.zero) 0 65 (k_opad VALS)),
-        `(array_at tuchar Tsh (fun _ : Z => Vint Int.zero) (Zlength (key a)) 65 (k_ipad VALS)),
-        `(data_at_ Tsh (tarray tuchar 32) (tk VALS)),
-        `(data_at_ Tsh (tarray tuchar 32) (tk2 VALS)),
-        `(data_at_ Tsh (tarray tuchar 1024) (bufferIn VALS)),
-        `(data_at_ Tsh (tarray tuchar 1024) (bufferOut VALS)),
-        `(K_vector KV),
-(*        `(array_at tuchar ksh (tuchars (map Int.repr (key a))) 0 (Zlength (key a))
-  (KEY A) * *)
-        `(memory_block dsh (Int.repr 32) (DIGEST A)),
-        `(repr_text a tsh (TEXT A))]).
-       subst Frame. reflexivity.
-     rewrite FR. clear FR Frame.
-     entailer.
-     rewrite HH2 in *. inversion H3; clear H3. subst keylen'. simpl in HH9.
-     assert (KeyLenRangeUnsigned :0 <= key_len a <= Int.max_unsigned).
-       rewrite int_max_unsigned_eq. 
-       destruct HH1 as [KLpos KLsignedBound].
-        rewrite int_max_signed_eq in KLsignedBound; omega.
-     rewrite Int.unsigned_repr in *; trivial.
-     rewrite (memory_block_array_tuchar' _ (key_len a)); trivial; try omega.
-     entailer. cancel.
-     rewrite <- HH9.
-     rewrite (split_array_at (Zlength (key a))).
-       2: rewrite HH9; omega.
-     cancel.
-     apply array_at_ext'. 
-        intros. unfold tuchars, cVint, ZnthV. simpl.
-          if_tac. omega.
-          destruct (nth_mapVintZ i (key a)) as [? I]; trivial.
-          rewrite I; reflexivity.
-   } 
-   after_call. 
-   (*Warning: Collision between bound variables of name x *)
-   subst WITNESS. normalize. subst retval1.
- 
-   
-   (**************** memcpy( k_opad, key, key_len ) ******)
-(*   frame_SEP does not apply for some reason*)
-   remember (ksh, Tsh, k_opad VALS, KEY A, key_len a,  
-            force_int oo (ZnthV tuchar (map Vint (map Int.repr (key a))))
-       ) as WITNESS. 
-   forward_call WITNESS.
-   { rewrite HeqWITNESS; clear HeqWITNESS WITNESS.
-     assert (FR: Frame = [
-      `(array_at tuchar Tsh
-        (fun i : Z =>
-         Vint (force_int (ZnthV tuchar (map Vint (map Int.repr (key a))) i))) 0
-        (key_len a) (k_ipad VALS)),
-      `(array_at tuchar Tsh (fun _ : Z => Vint Int.zero) (key_len a) 65 (k_ipad VALS)),
-      `(data_at_ Tsh (tarray tuchar 32) (tk VALS)),
-      `(data_at_ Tsh (tarray tuchar 32) (tk2 VALS)),
-      `(data_at_ Tsh (tarray tuchar 1024) (bufferIn VALS)),
-      `(data_at_ Tsh (tarray tuchar 1024) (bufferOut VALS)),
-      `(K_vector KV),
-      `(repr_text a tsh (TEXT A)),
-      `(memory_block dsh (Int.repr 32) (DIGEST A)),
-      `(array_at tuchar Tsh (fun _ : Z => Vint Int.zero) (key_len a) 65
-          (k_opad VALS))]).
-      subst Frame. reflexivity.
-     rewrite FR. clear FR Frame.
-     entailer.
-     rewrite HH2 in *. inversion H3; clear H3. subst keylen'. 
-     assert (KeyLenRangeUnsigned :0 <= key_len a <= Int.max_unsigned).
-       rewrite int_max_unsigned_eq. 
-       destruct HH1 as [KLpos KLsignedBound].
-        rewrite int_max_signed_eq in KLsignedBound; omega.
-     rewrite Int.unsigned_repr in *; trivial.
-     apply andp_right. abstract entailer.
-     cancel. 
-     rewrite (split_array_at (key_len a) tuchar Tsh _ 0 65 (k_opad VALS)).
-        2: omega. 
-     rewrite (memory_block_array_tuchar' _ (key_len a)); trivial.
-        2: omega.
-     rewrite HH9.
-     abstract cancel. 
-   } 
-   after_call. 
-   (*cbv beta iota.  autorewrite with norm subst. red. (* after_call. *)*)
-   (*Warning: Collision between bound variables of name x *)
-   subst WITNESS. normalize. 
-   subst retval1. 
-
-   (***************for -loop*********************)
-   unfold isPosSigned in HH1.
-   remember ((firstn (Z.to_nat (key_len a)) (key a)) ++ Nlist Z0 (65 - Z.to_nat (key_len a))) as normKey.
-   assert (LN: length normKey = 65%nat).
-     subst. rewrite app_length, firstn_length, length_Nlist.
-     clear - HH9 KLrange GT.
-     rewrite Zlength_correct in HH9; simpl in HH9. 
-     rewrite <- HH9, Nat2Z.id, Min.min_idempotent. omega.
-
-       assert (LK: (length (key a) <= 64)%nat).
-         rewrite <- HH9, Zlength_correct in GT. 
-         apply Z2Nat.inj_le in GT.
-         rewrite Nat2Z.id in GT. apply GT.
-         rewrite <- Zlength_correct. apply initial_world.zlength_nonneg.
-         omega.
-
-  eapply semax_seq'. 
-  frame_SEP 1 2 3 11. unfold isbyteZ in isByteKey.
-  forward_for_simple_bound 64 (EX i:Z, 
-  (PROP  ()
-   LOCAL  (
-    `(eq (TEXT A)) (eval_id _text); `(eq (KEY A)) (eval_id _key);
-   `(eq KV) (eval_var sha._K256 (tarray tuint 64));
-   `(eq (TEXTLEN A)) (eval_id _text_len);
-   `(eq (KEYLEN A)) (eval_id _key_len); `(eq (DIGEST A)) (eval_id _digest);
-   `(eq (k_ipad VALS)) (eval_var _k_ipad (tarray tuchar 65));
-   `(eq (k_opad VALS)) (eval_var _k_opad (tarray tuchar 65));
-   `(eq (tk VALS)) (eval_var _tk (tarray tuchar 32));
-   `(eq (tk2 VALS)) (eval_var _tk2 (tarray tuchar 32));
-   `(eq (bufferIn VALS)) (eval_var _bufferIn (tarray tuchar 1024));
-   `(eq (bufferOut VALS)) (eval_var _bufferOut (tarray tuchar 1024)))
-   SEP 
-   (
-   `(array_at tuchar Tsh
-       (cVint (force_int oo ZnthV tuchar (map Vint (map Int.repr (map Byte.unsigned (map Byte.repr (HMAC_FUN.mkKey (key a))))))))
-       i 64 (k_opad VALS));
-   `(array_at tuchar Tsh
-       (cVint (force_int oo ZnthV tuchar (map Vint (map Int.repr (map Byte.unsigned (map Byte.repr (HMAC_FUN.mkKey (key a))))))))
-       i 64 (k_ipad VALS));
-   `(array_at tuchar Tsh (fun _ : Z => Vint Int.zero)
-       64 65(k_opad VALS));
-   `(array_at tuchar Tsh (fun _ : Z => Vint Int.zero)
-       64 65 (k_ipad VALS));
-   `(array_at tuchar Tsh
-       (cVint (force_int oo ZnthV tuchar (map Vint (map Int.repr (map Byte.unsigned (HMAC_FUN.mkArg (map Byte.repr (HMAC_FUN.mkKey (key a))) Opad))))))
-       0 i (k_opad VALS));
-   `(array_at tuchar Tsh
-       (cVint (force_int oo ZnthV tuchar (map Vint (map Int.repr (map Byte.unsigned (HMAC_FUN.mkArg (map Byte.repr (HMAC_FUN.mkKey (key a))) Ipad))))))
-       0 i (k_ipad VALS))))).
-   
-   { (*precondition implies "invariant"*)
-     rewrite array_at_emp. rewrite array_at_emp. entailer.
-     apply andp_right. unfold array_at. abstract entailer.
-     repeat rewrite (map_map Byte.unsigned). 
-     assert (EQ: forall i : Z, 0 <= i < key_len a ->
-      cVint (force_int oo ZnthV tuchar (map Vint (map Int.repr (key a)))) i =
-      cVint (force_int oo ZnthV tuchar
-        (map Vint
-           (map (fun x : byte => Int.repr (Byte.unsigned x))
-              (map Byte.repr (key a))))) i).
-     { intros; unfold cVint. f_equal; simpl.
-       unfold ZnthV. destruct (zlt i 0); simpl; trivial.
-       assert (I: (0 <= Z.to_nat i < length (key a))%nat).
-         destruct H as [X Y]. 
-         apply Z2Nat.inj_lt in Y.
-         rewrite <- HH9, Zlength_correct, Nat2Z.id in Y. omega. omega. omega.
-       destruct (nth_mapVint (Z.to_nat i) (key a)); trivial.
-       rewrite H12. simpl. rewrite map_map. rewrite map_map.
-       rewrite <- nth_default_eq in H12. unfold nth_default in H12.
-       remember (nth_error (map Vint (map Int.repr (key a))) (Z.to_nat i)) as d. 
-       destruct d; inversion H12. clear H12; subst v. 
-       apply eq_sym in Heqd. destruct (map_nth_error_inv _ _ _  _ Heqd) as [? [? ?]].
-       inv H13; clear Heqd. destruct (map_nth_error_inv _ _ _  _ H12) as [? [? ?]]. subst x0; clear H12.
-       rewrite nth_map' with (d':=Z0). 
-       rewrite <- nth_default_eq. unfold nth_default. rewrite H13.
-       rewrite Byte.unsigned_repr. trivial.
-       rewrite Forall_forall in isByteKey. 
-       apply nth_error_in in H13. apply isByteKey in H13.
-         unfold Byte.max_unsigned, Byte.modulus, Byte.wordsize. simpl. omega.
-       apply I.
-     }
-     rewrite (split_array_at 64 tuchar Tsh _ (key_len a) 65); try omega.
-     rewrite (split_array_at 64 tuchar Tsh _ (key_len a) 65); try omega.
-     cancel.
-     rewrite (split_array_at (key_len a) tuchar Tsh _ 0 64); try omega.
-     rewrite (split_array_at (key_len a) tuchar Tsh _ 0 64); try omega.
-     repeat rewrite sepcon_assoc.
-     apply sepcon_derives. apply array_at_ext'. 
-       intros. rewrite EQ; trivial. unfold cVint; simpl. f_equal. f_equal.
-       unfold ZnthV. if_tac. omega. simpl. clear H12.
-       assert (I: (0 <= Z.to_nat i < length (key a))%nat).
-         destruct H as [X Y]. 
-         apply Z2Nat.inj_lt in Y.
-         rewrite <- HH9, Zlength_correct, Nat2Z.id in Y. omega. omega. omega.
-       assert (X: (Z.to_nat i < length (HMAC_FUN.mkKey (key a)))%nat).
-         rewrite HMAC_FUN.mkKey_length. unfold SHA256_BlockSize. omega.
-       repeat rewrite nth_map' with (d':=Int.zero); try repeat rewrite map_length; try omega.
-       f_equal.
-       repeat rewrite nth_map' with (d':=Byte.zero); try repeat rewrite map_length; try omega.
-       f_equal. f_equal.
-         rewrite <- HH9 in H, HeqKLENGTH.
-       repeat rewrite nth_map' with (d':=Z0); try repeat rewrite map_length; try omega.
-       f_equal.
-         erewrite mkKey_left; trivial.
-     rewrite <- sepcon_assoc.
-     apply cancel1_last. apply array_at_ext'.
-       clear - KLrange HH9 HeqKLENGTH.
-       intros. unfold cVint; simpl. f_equal. 
-       unfold ZnthV. if_tac. omega. 
-       assert (X: (Z.to_nat i < length (HMAC_FUN.mkKey (key a)))%nat).
-         rewrite HMAC_FUN.mkKey_length. unfold SHA256_BlockSize.
-         destruct H as [X Y].  apply Z2Nat.inj_lt in Y. apply Y. omega. omega.
-       repeat rewrite nth_map' with (d':=Int.zero); try repeat rewrite map_length; try omega.
-       f_equal.
-       repeat rewrite nth_map' with (d':=Byte.zero); try repeat rewrite map_length; try omega.
-       f_equal. f_equal.
-         rewrite <- HH9 in H, HeqKLENGTH.
-       rewrite nth_map' with (d':=Z0); try repeat rewrite map_length; try omega.
-       rewrite mkKey_right; trivial. 
-     apply sepcon_derives. apply array_at_ext'. 
-       intros. unfold cVint in *. simpl in EQ. rewrite EQ; trivial. simpl. f_equal. f_equal.
-       unfold ZnthV. if_tac. omega. simpl. 
-       assert (I: (0 <= Z.to_nat i < length (key a))%nat).
-         destruct H as [X Y]. 
-         apply Z2Nat.inj_lt in Y.
-         rewrite <- HH9, Zlength_correct, Nat2Z.id in Y. omega. omega. omega.
-       assert (X: (Z.to_nat i < length (HMAC_FUN.mkKey (key a)))%nat).
-         rewrite HMAC_FUN.mkKey_length. unfold SHA256_BlockSize. omega.
-       repeat rewrite nth_map' with (d':=Int.zero); try repeat rewrite map_length; try omega.
-       f_equal.
-       repeat rewrite nth_map' with (d':=Byte.zero); try repeat rewrite map_length; try omega.
-       f_equal. f_equal.
-         rewrite <- HH9 in H, HeqKLENGTH.
-       repeat rewrite nth_map' with (d':=Z0); try repeat rewrite map_length; try omega.
-       f_equal.
-         erewrite mkKey_left; trivial.
-     apply array_at_ext'. 
-       intros. clear EQ. unfold cVint; simpl. f_equal. 
-       unfold ZnthV. if_tac. omega. 
-       assert (X: (Z.to_nat i < length (HMAC_FUN.mkKey (key a)))%nat).
-         rewrite HMAC_FUN.mkKey_length. unfold SHA256_BlockSize.
-         destruct H as [X Y].  apply Z2Nat.inj_lt in Y. apply Y. omega. omega.
-       repeat rewrite nth_map' with (d':=Int.zero); try repeat rewrite map_length; try omega.
-       f_equal.
-       repeat rewrite nth_map' with (d':=Byte.zero); try repeat rewrite map_length; try omega.
-       f_equal. f_equal.
-         rewrite <- HH9 in H, HeqKLENGTH.
-       rewrite nth_map' with (d':=Z0); try repeat rewrite map_length; try omega.
-       rewrite mkKey_right; trivial. 
-   }
-   { (*show that body satisfies "invariant"*)
-     admit. (*
-     hoist_later_in_pre.
-     simple eapply semax_seq'.
-     remember (cVint
-             (force_int
-              oo ZnthV tuchar
-                   (map Vint
-                      (map Int.repr
-                         (map Byte.unsigned
-                            (map Byte.repr (HMAC_FUN.mkKey (key a)))))))) as KKEY.
-     remember (cVint
-            (force_int
-             oo ZnthV tuchar
-                  (map Vint
-                     (map Int.repr
-                        (map Byte.unsigned
-                           (HMAC_FUN.mkArg
-                              (map Byte.repr (HMAC_FUN.mkKey (key a))) Opad)))))) as OPAD.
-     remember (cVint
-            (force_int
-             oo ZnthV tuchar
-                  (map Vint
-                     (map Int.repr
-                        (map Byte.unsigned
-                           (HMAC_FUN.mkArg
-                              (map Byte.repr (HMAC_FUN.mkKey (key a))) Ipad)))))) as IPAD.
-      remember (Ederef
-        (Ebinop Oadd (Evar _k_ipad (tarray tuchar 65)) (Etempvar _i tint)
-           (tptr tuchar)) tuchar) as e1.
-        eapply semax_loadstore_array'.
-assert (typeof e1 = tuchar). subst e1. simpl. reflexivity.
-      remember (Ederef
-        (Ebinop Oadd (Evar _k_ipad (tptr tuchar)) (Etempvar _i tint)
-           (tptr tuchar)) tuchar) as e1'.
-assert (typeof e1' = tuchar). subst e1'. simpl. reflexivity.
-          reflexivity. apply I. reflexivity.
-        Focus 8. entailer. 
-          repeat apply andp_right. 
-         (*rel_expr (Evar _k_ipad (tarray tuchar 65)) ?7539 rho*)
-          Focus 2. eapply rel_expr_cast.
-                   eapply rel_expr_binop.
-          instantiate (1:= k_ipad VALS). rel_expr. unfold eval_var in H7.
-          Focus 2. rel_expr.
-          Focus 2. eapply rel_expr_cast.
-                   eapply rel_expr_binop. 
-                   (* rel_expr
-(*        eapply semax_loadstore_array.?*)
-          reflexivity. apply I. reflexivity. admit. (*TODO tarray/tptr*)
-          reflexivity. 
-        entailer. 
-          repeat apply andp_right. 
-         (*rel_expr (Evar _k_ipad (tarray tuchar 65)) ?7539 rho*)
-          instantiate (1:= k_ipad VALS). rel_expr. unfold eval_var in H7.
-          Focus 2. rel_expr.
-          Focus 2. eapply rel_expr_cast.
-                   eapply rel_expr_binop. 
-                   (* rel_expr
-      (Ederef
-         (Ebinop *)
-                  Focus 2. rel_expr. 
-                  Focus 2. simpl. eapply rel_expr_deref.
-                  rel_expr. auto.
-                apply andp_right. 
-SearchAbout rel_lvalue. rel_expr. 
-           eapply rel_expr_array_load'.
-       reflexivity. apply I. reflexivity.
-     simple eapply semax_loadstore_array.
-       reflexivity. apply I. reflexivity.
-       unfold tarray; simpl. admit. (*TODO: refine Lemma semax_loadstore_array' in array_lemmas.v*)
-       reflexivity.
-     *)*)
-   }
-(*NEW OUT-OF_MEMORY-CRASH emerged here (in the next 5 lines) in svn version 6738 (or a bit before that, since I hadnt updated for a couple of days)*)
-   { (*show increment*) trivial. }
-   clear LN HeqnormKey normKey.
-
-   (*normalize. *) unfold update_tycon; simpl.
-   repeat rewrite array_at_emp; simpl.
-
-Require Import HMAC_proofTail. rewrite Zplus_comm in TL1024.
-specialize (hmac_LE_tail Espec tsh ksh dsh A a KV text' key' digest' textlen'
-  keylen' perms h0 l Heql Heqh0 VALS HeqKLENGTH GT H0 HH1 HH2 HH3 HH4 TL1024
-  HH5 HH6 HH7 HH8 HH9 TLrange KLrange isByteKey LK).
-intros TAIL.
-abstract solve [apply TAIL].
-(*apply hmac_LE_tail.*)
-(*
- unfold MORE_COMMANDS, abbreviate. xx normalize. (*WHY are the two `emp terms not eliminated here???*)
-
-(****************** continuation after for-loop **************************)
- remember (map Byte.unsigned
-                         (HMAC_FUN.mkArg
-                            (map Byte.repr (HMAC_FUN.mkKey (key a))) Ipad))
-     as KIPAD.
- remember (force_int
-           oo ZnthV tuchar
-                (map Vint (map Int.repr KIPAD))) as IPAD.
- remember (map Byte.unsigned
-                         (HMAC_FUN.mkArg
-                            (map Byte.repr (HMAC_FUN.mkKey (key a))) Opad))
-     as KOPAD.
- remember (force_int
-           oo ZnthV tuchar
-                (map Vint (map Int.repr KOPAD))) as OPAD.
-  remember (force_int oo ZnthV tuchar (map Vint (map Int.repr (key a)))) as KKEY. 
- remember (fun _ : Z => Vint Int.zero) as ZERO.
- normalize. 
-
- eapply restLE; eassumption.
-*)
+   admit.
 }
 Qed.
