sha/HMAC_lemmas.v
@@ -1,0 +1,150 @@
+Require Import floyd.proofauto.
+
+Import ListNotations.
+Local Open Scope logic.
+Require Import sha.spec_sha.
+Require Import sha.HMAC_functional_prog.
+
+Lemma In_Nlist {A:Type}: forall (n:A) l x, In x (Nlist n l) -> x=n.
+Proof. intros n l.
+  induction l; simpl; intros. contradiction.
+  destruct H; eauto.
+Qed.
+Lemma zeropad_isbyteZ: forall l, Forall isbyteZ l -> Forall isbyteZ (HMAC_FUN.zeroPad l).
+Proof. unfold isbyteZ, HMAC_FUN.zeroPad; intros.
+  rewrite Forall_forall in *. intros.
+  apply in_app_or in H0.
+  destruct H0. apply (H _ H0).
+  apply In_Nlist in H0. subst; omega.
+Qed.
+Lemma mapnth': forall {A B : Type} (f : A -> B) (l : list A) (d : A) (n : nat) fd,
+      fd = f d -> nth n (map f l) fd = f (nth n l d).
+Proof. intros; subst. apply map_nth. Qed.
+Lemma map_unsigned_Brepr_isbyte: forall l, Forall isbyteZ l ->
+      map Byte.unsigned (map Byte.repr l) = l.
+Proof. intros. induction l; simpl in *. trivial.
+   rewrite IHl. rewrite Byte.unsigned_repr. trivial. 
+   rewrite Forall_forall in H. 
+   assert (In a (a::l)). left. trivial. 
+   specialize (H _ H0); clear H0.
+      unfold isbyteZ in H. unfold Byte.max_unsigned, Byte.modulus. simpl. omega.
+   rewrite Forall_forall in *. intros. apply H. right; trivial.
+Qed.
+Lemma Ztest_Bytetest:
+ forall a, Z.testbit (Byte.unsigned a) = Byte.testbit a.
+Proof. reflexivity. Qed.
+Hint Rewrite Ztest_Bytetest : testbit.
+
+Lemma nthD_1 {A B}: forall (f: A ->B) n l d fx dd, (n < length l)%nat ->
+      nth n (map f l) d = fx -> 
+      exists x, In x l /\ nth n l dd = x /\ f x = fx.
+Proof. intros f n.
+  induction n; simpl; intros.
+    destruct l; simpl in *. omega.
+      exists a; split. left; trivial. split; trivial.
+    destruct l; simpl in *. omega. 
+    destruct (IHn l d fx dd) as [? [? [? ?]]]. omega. trivial.
+    exists x; eauto.
+Qed.
+
+(*Same proof as semax_loadstore_array*)
+Lemma NEWsemax_loadstore_array:
+  forall {Espec: OracleKind},
+ forall n k vi lo hi t1 (contents: Z -> reptype t1) v1 v2 (Delta: tycontext) e1 ei e2 sh P Q R, 
+  (*H0*) reptype t1 = val -> 
+  (*H1*) type_is_by_value t1 ->
+  (*H2*) legal_alignas_type t1 = true ->
+  (*H3*) typeof e1 = tarray t1 k->
+  (*H4*) typeof ei = tint ->
+  (*H8*) PROPx P (LOCALx Q (SEPx R)) |--  rel_expr e1 v1 && rel_expr ei (Vint (Int.repr vi))
+           && rel_expr (Ecast e2 t1) v2 ->
+  (*H7*) nth_error R n = Some (`(array_at t1 sh contents lo hi v1)) ->
+  (*H *) writable_share sh ->
+  (*H5*) tc_val t1 v2 ->
+  (*H6*) in_range lo hi vi ->
+   @semax Espec Delta (|> PROPx P (LOCALx Q (SEPx R))) (Sassign (Ederef (Ebinop Oadd e1 ei (tptr t1)) t1) e2) 
+          (normal_ret_assert 
+           (PROPx P (LOCALx Q (SEPx 
+            (replace_nth n R `(array_at t1 sh (upd contents vi (valinject _ v2)) lo hi v1)))))).
+Proof. 
+intros until R.
+intros H0 H1 H2 H3 H4 H8 H7 H H5 H6.
+eapply semax_post_flipped'.
+apply semax_loadstore_array'; eauto.
+apply derives_trans with (!! isptr v1 && PROPx P (LOCALx Q (SEPx R))).
+rewrite (SEP_nth_isolate _ _ _ H7).
+repeat rewrite <- insert_SEP.
+rewrite array_at_isptr. normalize.
+normalize.
+destruct v1; try contradiction.
+instantiate (2:=v1).
+simpl eval_binop. rewrite mul_repr.
+apply andp_right; auto.
+eapply derives_trans; [ apply H8 |].
+intro rho. simpl.
+repeat apply andp_right.
+apply rel_lvalue_deref.
+eapply rel_expr_binop.
+repeat apply andp_left1. apply derives_refl.
+apply andp_left1. apply andp_left2. apply derives_refl.
+intro; rewrite H4; simpl. rewrite H3; simpl. 
+  unfold Cop.sem_add; simpl. rewrite mul_repr. auto.
+ apply andp_left2. auto.
+rewrite (SEP_nth_isolate _ _ _ H7).
+repeat rewrite <- insert_SEP.
+apply derives_refl.
+rewrite (SEP_replace_nth_isolate _ _ _ `(array_at t1 sh (upd contents vi (valinject t1 v2)) lo hi v1) H7).
+rewrite insert_SEP.
+auto.
+Qed.
+
+Lemma array_at_local_facts':
+  forall (t : type) (sh : Share.t) (f : Z -> reptype t) (lo hi : Z) (v : val),
+  array_at t sh f lo hi v |-- array_at t sh f lo hi v && !!isptr v && !!offset_in_range (sizeof t * lo) v &&
+!!offset_in_range (sizeof t * hi) v && !!align_compatible t v.
+Proof. intros. unfold array_at. entailer. Qed.
+
+
+Lemma split_offset_array_at_: forall (ty : type) (sh : Share.t) 
+         (z lo hi : Z) (v : val),
+       z <= lo <= hi ->
+       sizeof ty > 0 ->
+       legal_alignas_type ty = true ->
+       array_at_ ty sh z hi v =
+       !! offset_in_range (sizeof ty * z) v &&
+       !! offset_in_range (sizeof ty * hi) v &&
+       array_at_ ty sh z lo v * 
+       array_at_ ty sh 0 (hi - lo) 
+       (offset_val (Int.repr (sizeof ty * lo)) v).
+Proof.
+  intros. unfold array_at_.
+  rewrite <- split_offset_array_at; trivial.
+Qed.
+Lemma offset_val_array_at0:
+ forall t sh f lo hi v,
+  sizeof t > 0 -> hi >= 0 ->
+  legal_alignas_type t = true ->
+  array_at t sh (fun i => f (i-lo)%Z) lo (lo + hi) v 
+  |--
+  array_at t sh f 0 hi (offset_val (Int.repr (sizeof t * lo)) v).
+Proof.
+  intros.
+  rewrite (split_offset_array_at t _ _ lo lo); trivial.
+  rewrite array_at_emp.
+  entailer. rewrite Zplus_comm. rewrite Z.add_simpl_r.
+  apply array_at_ext'. intros. rewrite Z.add_simpl_r. trivial.
+  omega.
+Qed.
+
+Lemma offset_val_array_at1:
+ forall t sh f g k lo hi ofs v,
+    sizeof t > 0 -> hi >= 0 ->
+    legal_alignas_type t = true ->
+    k = lo + hi ->
+    g = (fun i => f (i-lo)%Z) ->
+    ofs = Int.repr (sizeof t * lo) ->
+  array_at t sh g lo k v |--
+  array_at t sh f 0 hi ((offset_val ofs) v).
+Proof.
+  intros. subst. apply offset_val_array_at0; trivial.
+Qed.
