sha/HMAC_proofLE.v
@@ -1,0 +1,1186 @@
+Require Import floyd.proofauto.
+
+Import ListNotations.
+Require sha.sha.
+Require sha.SHA256.
+Local Open Scope logic.
+
+Require Import sha.spec_sha.
+
+Require Import sha.HMAC_functional_prog.
+Require Import sha.HMAC_refined_fp.
+
+Require Import sha.hmac_sha256.
+
+Require Import HMAC_definitions.
+(*Require Import HMAC_part2LE. this file contains the implementation for the path key_len <= 64*)
+(*Require Import HMAC_part2GT. this file contains the implementation for the path key_len > 64*)
+
+Declare Module PART2LE: HMAC_PART2LE.
+(*Declare Module PART2GT: HMAC_PART2GT.*)
+
+Definition restLE := PART2LE.HMAC_LE.
+(*Definition restGT := PART2GT.HMAC_GT.*)
+
+Require Import HMAC_LoopBodyLE.
+(*
+Lemma caseLE Espec tsh ksh dsh : forall
+(A : ARGS)
+(a : HMAC_Refined.Args)
+(KV : val) argshares
+(HAS: argshares = (tsh, (ksh, dsh)))
+(H : prop_args argshares A a)
+(*Struct_env := abbreviate : type_id_env*)
+(text' : name _text)
+(key' : name _key)
+(digest' : name _digest)
+(textlen' : name _text_len)
+(keylen' : name _key_len)
+(perms : permissions)
+(h0 : HMAC_Refined.hmacState)
+(Heqh0 : h0 =
+        {|
+        HMAC_Refined.args := a;
+        HMAC_Refined.locals := HMAC_Refined.initLocalVals |})
+(VALS : VALUES)
+(h1 : HMAC_Refined.hmacState)
+(Heqh1 : h1 = HMAC_Refined.snippet1 h0)
+(HeqKLENGTH : false = (key_len a >? 64))
+(GT : key_len a <= 64)
+(H0 : sizes)
+(Delta := func_tycontext f_hmac_sha256 Vprog Gtot)
+(*POSTCONDITION := abbreviate : ret_assert
+MORE_COMMANDS := abbreviate : statement*),
+@semax Espec Delta
+  (PROP  ()
+   LOCAL  (`(eq (TEXT A)) (eval_id _text); `(eq (KEY A)) (eval_id _key);
+   `(eq KV) (eval_var sha._K256 (tarray tuint 64));
+   `(eq (TEXTLEN A)) (eval_id _text_len);
+   `(eq (KEYLEN A)) (eval_id _key_len); `(eq (DIGEST A)) (eval_id _digest);
+   `(eq (k_ipad VALS)) (eval_var _k_ipad (tarray tuchar 65));
+   `(eq (k_opad VALS)) (eval_var _k_opad (tarray tuchar 65));
+   `(eq (tk VALS)) (eval_var _tk (tarray tuchar 32));
+   `(eq (tk2 VALS)) (eval_var _tk2 (tarray tuchar 32));
+   `(eq (bufferIn VALS)) (eval_var _bufferIn (tarray tuchar 1024));
+   `(eq (bufferOut VALS)) (eval_var _bufferOut (tarray tuchar 1024)))
+   SEP  (`(data_at_ Tsh (tarray tuchar 65) (k_ipad VALS));
+   `(data_at_ Tsh (tarray tuchar 65) (k_opad VALS));
+   `(repr_local (negb false) Tsh (tarray tuchar 32) (tk (locals h1))
+       (tk VALS)); `(data_at_ Tsh (tarray tuchar 32) (tk2 VALS));
+   `(data_at_ Tsh (tarray tuchar 1024) (bufferIn VALS));
+   `(data_at_ Tsh (tarray tuchar 1024) (bufferOut VALS)); `(K_vector KV);
+   `(repr_args argshares A a true)))
+  (Ssequence
+     (Scall None
+        (Evar _memset
+           (Tfunction (Tcons (tptr tvoid) (Tcons tint (Tcons tuint Tnil)))
+              (tptr tvoid) cc_default))
+        [Evar _k_ipad (tarray tuchar 65), Econst_int (Int.repr 0) tint,
+        Econst_int (Int.repr 65) tuint])
+     (Ssequence
+        (Scall None
+           (Evar _memset
+              (Tfunction (Tcons (tptr tvoid) (Tcons tint (Tcons tuint Tnil)))
+                 (tptr tvoid) cc_default))
+           [Evar _k_opad (tarray tuchar 65), Econst_int (Int.repr 0) tint,
+           Econst_int (Int.repr 65) tuint])
+        (Ssequence
+           (Scall None
+              (Evar _memcpy
+                 (Tfunction
+                    (Tcons (tptr tvoid)
+                       (Tcons (tptr tvoid) (Tcons tuint Tnil))) (tptr tvoid)
+                    cc_default))
+              [Evar _k_ipad (tarray tuchar 65), Etempvar _key (tptr tuchar),
+              Etempvar _key_len tint])
+           (Ssequence
+              (Scall None
+                 (Evar _memcpy
+                    (Tfunction
+                       (Tcons (tptr tvoid)
+                          (Tcons (tptr tvoid) (Tcons tuint Tnil)))
+                       (tptr tvoid) cc_default))
+                 [Evar _k_opad (tarray tuchar 65),
+                 Etempvar _key (tptr tuchar), Etempvar _key_len tint])
+              (Ssequence
+                 (Ssequence (Sset _i (Econst_int (Int.repr 0) tint))
+                    (Sloop
+                       (Ssequence
+                          (Sifthenelse
+                             (Ebinop Olt (Etempvar _i tint)
+                                (Econst_int (Int.repr 64) tint) tint) Sskip
+                             Sbreak)
+                          (Ssequence
+                             (Sassign
+                                (Ederef
+                                   (Ebinop Oadd
+                                      (Evar _k_ipad (tarray tuchar 65))
+                                      (Etempvar _i tint) (tptr tuchar))
+                                   tuchar)
+                                (Ebinop Oxor
+                                   (Ederef
+                                      (Ebinop Oadd
+                                         (Evar _k_ipad (tarray tuchar 65))
+                                         (Etempvar _i tint) (tptr tuchar))
+                                      tuchar) (Econst_int (Int.repr 54) tint)
+                                   tint))
+                             (Sassign
+                                (Ederef
+                                   (Ebinop Oadd
+                                      (Evar _k_opad (tarray tuchar 65))
+                                      (Etempvar _i tint) (tptr tuchar))
+                                   tuchar)
+                                (Ebinop Oxor
+                                   (Ederef
+                                      (Ebinop Oadd
+                                         (Evar _k_opad (tarray tuchar 65))
+                                         (Etempvar _i tint) (tptr tuchar))
+                                      tuchar) (Econst_int (Int.repr 92) tint)
+                                   tint))))
+                       (Sset _i
+                          (Ebinop Oadd (Etempvar _i tint)
+                             (Econst_int (Int.repr 1) tint) tint))))
+                 (Ssequence
+                    (Scall None
+                       (Evar _memset
+                          (Tfunction
+                             (Tcons (tptr tvoid)
+                                (Tcons tint (Tcons tuint Tnil))) (tptr tvoid)
+                             cc_default))
+                       [Evar _bufferIn (tarray tuchar 1024),
+                       Econst_int (Int.repr 0) tint,
+                       Econst_int (Int.repr 1024) tint])
+                    (Ssequence
+                       (Scall None
+                          (Evar _memcpy
+                             (Tfunction
+                                (Tcons (tptr tvoid)
+                                   (Tcons (tptr tvoid) (Tcons tuint Tnil)))
+                                (tptr tvoid) cc_default))
+                          [Evar _bufferIn (tarray tuchar 1024),
+                          Evar _k_ipad (tarray tuchar 65),
+                          Econst_int (Int.repr 64) tint])
+                       (Ssequence
+                          (Scall None
+                             (Evar _memcpy
+                                (Tfunction
+                                   (Tcons (tptr tvoid)
+                                      (Tcons (tptr tvoid) (Tcons tuint Tnil)))
+                                   (tptr tvoid) cc_default))
+                             [Ebinop Oadd
+                                (Evar _bufferIn (tarray tuchar 1024))
+                                (Econst_int (Int.repr 64) tint) (tptr tuchar),
+                             Etempvar _text (tptr tuchar),
+                             Etempvar _text_len tint])
+                          (Ssequence
+                             (Scall None
+                                (Evar _SHA256
+                                   (Tfunction
+                                      (Tcons (tptr tuchar)
+                                         (Tcons tuint
+                                            (Tcons (tptr tuchar) Tnil)))
+                                      tvoid cc_default))
+                                [Evar _bufferIn (tarray tuchar 1024),
+                                Ebinop Oadd (Econst_int (Int.repr 64) tint)
+                                  (Etempvar _text_len tint) tint,
+                                Evar _tk2 (tarray tuchar 32)])
+                             (Ssequence
+                                (Scall None
+                                   (Evar _memset
+                                      (Tfunction
+                                         (Tcons (tptr tvoid)
+                                            (Tcons tint (Tcons tuint Tnil)))
+                                         (tptr tvoid) cc_default))
+                                   [Evar _bufferOut (tarray tuchar 1024),
+                                   Econst_int (Int.repr 0) tint,
+                                   Econst_int (Int.repr 1024) tint])
+                                (Ssequence
+                                   (Scall None
+                                      (Evar _memcpy
+                                         (Tfunction
+                                            (Tcons (tptr tvoid)
+                                               (Tcons (tptr tvoid)
+                                                  (Tcons tuint Tnil)))
+                                            (tptr tvoid) cc_default))
+                                      [Evar _bufferOut (tarray tuchar 1024),
+                                      Evar _k_opad (tarray tuchar 65),
+                                      Econst_int (Int.repr 64) tint])
+                                   (Ssequence
+                                      (Scall None
+                                         (Evar _memcpy
+                                            (Tfunction
+                                               (Tcons (tptr tvoid)
+                                                  (Tcons (tptr tvoid)
+                                                     (Tcons tuint Tnil)))
+                                               (tptr tvoid) cc_default))
+                                         [Ebinop Oadd
+                                            (Evar _bufferOut
+                                               (tarray tuchar 1024))
+                                            (Econst_int (Int.repr 64) tint)
+                                            (tptr tuchar),
+                                         Evar _tk2 (tarray tuchar 32),
+                                         Econst_int (Int.repr 32) tint])
+                                      (Ssequence
+                                         (Scall None
+                                            (Evar _SHA256
+                                               (Tfunction
+                                                  (Tcons (tptr tuchar)
+                                                     (Tcons tuint
+                                                        (Tcons (tptr tuchar)
+                                                           Tnil))) tvoid
+                                                  cc_default))
+                                            [Evar _bufferOut
+                                               (tarray tuchar 1024),
+                                            Ebinop Oadd
+                                              (Econst_int (Int.repr 64) tint)
+                                              (Econst_int (Int.repr 32) tint)
+                                              tint,
+                                            Etempvar _digest (tptr tvoid)])
+                                         (Sreturn None))))))))))))))
+  (frame_ret_assert
+     (function_body_ret_assert tvoid
+        SEP  (`(K_vector KV); `(repr_key a ksh (KEY A));
+        `(repr_text a tsh (TEXT A));
+        `(repr_digest false (fst (RefinedHMAC a)) dsh (DIGEST A))))
+     (stackframe_of f_hmac_sha256)).
+Proof.
+intros.
+  remember (frame_ret_assert
+     (function_body_ret_assert tvoid
+        SEP  (`(K_vector KV); `(repr_key a ksh (KEY A));
+        `(repr_text a tsh (TEXT A));
+        `(repr_digest false (fst (RefinedHMAC a)) dsh (DIGEST A))))
+     (stackframe_of f_hmac_sha256))
+   as POSTCOND.
+
+  unfold HMAC_Refined.snippet1; simpl.
+  remember (HMAC_Refined.initLocalVals).  
+  assert (Heq: h1 = h0). 
+    subst h1. subst h0. 
+         unfold HMAC_Refined.snippet1; simpl.
+         rewrite <- HeqKLENGTH. reflexivity.
+  clear Heqh1. subst h1.
+  subst argshares. clear Heqh0 h0 Heql l.
+  destruct H as [[HH1 HH2] [[HH3 [HH4 TL1024]] [HH5 [HH6 [HH7 [HH8 HH9]]]]]].
+  rewrite HH4 in *.
+  assert (TLrange: 0 <= text_len a <= Int.max_unsigned).
+    clear - HH3. destruct HH3.
+    rewrite int_max_signed_eq in H0. rewrite int_max_unsigned_eq. omega.
+  simpl in HH8. rewrite Int.unsigned_repr in HH8; trivial.
+  assert (KLrange: 0 <= key_len a <= Int.max_unsigned).
+    clear - HH1. destruct HH1.
+    rewrite int_max_signed_eq in H0. rewrite int_max_unsigned_eq. omega.
+  rewrite HH2 in HH9; simpl in HH9.
+    rewrite Int.unsigned_repr in HH9; trivial.
+
+  remember (Tsh, k_ipad VALS, 65, Int.zero) as WITNESS.
+  forward_call (* memset *) WITNESS.
+  { assert (FR: Frame = [
+        `(data_at_ Tsh (tarray tuchar 65) (k_opad VALS)),
+        `(data_at_ Tsh (tarray tuchar 32) (tk VALS)),
+        `(data_at_ Tsh (tarray tuchar 32) (tk2 VALS)),
+        `(data_at_ Tsh (tarray tuchar 1024) (bufferIn VALS)),
+        `(data_at_ Tsh (tarray tuchar 1024) (bufferOut VALS)), 
+        `(K_vector KV),
+        `(repr_key a ksh (KEY A)),
+        `(repr_text a tsh (TEXT A)),
+        `(memory_block dsh (Int.repr 32) (DIGEST A))]).  
+      subst Frame. reflexivity. 
+    rewrite FR. clear FR Frame.
+    unfold repr_locals; simpl. intros rho.
+    entailer.
+    apply andp_right.
+      rewrite <- H6; clear H6. simpl.
+      rewrite (data_at__isptr _ _ (k_ipad VALS)). abstract entailer.
+    assert (SF: Int.repr 65 = Int.repr (sizeof (tarray tuchar 65))) by reflexivity.
+    rewrite SF, align_1_memory_block_data_at_; trivial.
+   }
+   after_call. 
+   (*Warning: Collision between bound variables of name x *)
+
+  forward_call (* memset *) (Tsh, k_opad VALS, 65, Int.zero).
+  { assert (FR: Frame = [
+        `(array_at tuchar Tsh (fun _ : Z => Vint Int.zero) 0 65 (k_ipad VALS)),
+        `(data_at_ Tsh (tarray tuchar 32) (tk VALS)),
+        `(data_at_ Tsh (tarray tuchar 32) (tk2 VALS)),
+        `(data_at_ Tsh (tarray tuchar 1024) (bufferIn VALS)),
+        `(data_at_ Tsh (tarray tuchar 1024) (bufferOut VALS)), 
+        `(K_vector KV),
+        `(repr_key a ksh (KEY A)),
+        `(repr_text a tsh (TEXT A)),
+        `(memory_block dsh (Int.repr 32) (DIGEST A))]).  
+      subst Frame. reflexivity.
+    rewrite FR. clear FR Frame.
+    unfold repr_locals; simpl. intros rho.
+    entailer.
+    apply andp_right.
+      rewrite <- H7; clear H7. simpl.
+      rewrite (data_at__isptr _ _ (k_opad VALS)). abstract entailer.
+    assert (SF: Int.repr 65 = Int.repr (sizeof (tarray tuchar 65))) by reflexivity.
+    rewrite SF, align_1_memory_block_data_at_; trivial. abstract cancel.
+   }
+   after_call. 
+   (*Warning: Collision between bound variables of name x *) 
+   subst retval1.
+
+   (**************** memcpy( k_ipad, key, key_len ) ******)
+   unfold repr_key, data_block. 
+   eapply semax_pre with (P' :=(PROP (Forall isbyteZ (key a))
+   LOCAL  (
+   `(eq (TEXT A)) (eval_id _text); `(eq (KEY A)) (eval_id _key);
+   `(eq KV) (eval_var sha._K256 (tarray tuint 64));
+   `(eq (TEXTLEN A)) (eval_id _text_len);
+   `(eq (KEYLEN A)) (eval_id _key_len); `(eq (DIGEST A)) (eval_id _digest);
+   `(eq (k_ipad VALS)) (eval_var _k_ipad (tarray tuchar 65));
+   `(eq (k_opad VALS)) (eval_var _k_opad (tarray tuchar 65));
+   `(eq (tk VALS)) (eval_var _tk (tarray tuchar 32));
+   `(eq (tk2 VALS)) (eval_var _tk2 (tarray tuchar 32));
+   `(eq (bufferIn VALS)) (eval_var _bufferIn (tarray tuchar 1024));
+   `(eq (bufferOut VALS)) (eval_var _bufferOut (tarray tuchar 1024)))
+   SEP 
+   (`(array_at tuchar Tsh (fun _ : Z => Vint Int.zero) 0 65 (k_opad VALS));
+   `(array_at tuchar Tsh (fun _ : Z => Vint Int.zero) 0 65 (k_ipad VALS));
+   `(data_at_ Tsh (tarray tuchar 32) (tk VALS));
+   `(data_at_ Tsh (tarray tuchar 32) (tk2 VALS));
+   `(data_at_ Tsh (tarray tuchar 1024) (bufferIn VALS));
+   `(data_at_ Tsh (tarray tuchar 1024) (bufferOut VALS)); `(K_vector KV);
+   `(array_at tuchar ksh (tuchars (map Int.repr (key a))) 0 (Zlength (key a))
+       (KEY A)); `(repr_text a tsh (TEXT A));
+   `(memory_block dsh (Int.repr 32) (DIGEST A))))).
+     abstract entailer. 
+
+   normalize. rename H1 into isByteKey.
+
+   (* following this recipe doesn't quite work, since some rewrite rule is missing to cleanup
+      the postcondition after after_call
+   eapply semax_seq'.
+   frame_SEP 7 1.*)
+   remember (ksh, Tsh, k_ipad VALS, KEY A, key_len a, 
+            force_int oo (ZnthV tuchar (map Vint (map Int.repr (key a))))
+       ) as WITNESS. 
+   forward_call (* memcopy *) WITNESS.
+   { rewrite HeqWITNESS; clear HeqWITNESS WITNESS.
+     assert (FR: Frame =
+       [`(array_at tuchar Tsh (fun _ : Z => Vint Int.zero) 0 65 (k_opad VALS)),
+        `(array_at tuchar Tsh (fun _ : Z => Vint Int.zero) (Zlength (key a)) 65 (k_ipad VALS)),
+        `(data_at_ Tsh (tarray tuchar 32) (tk VALS)),
+        `(data_at_ Tsh (tarray tuchar 32) (tk2 VALS)),
+        `(data_at_ Tsh (tarray tuchar 1024) (bufferIn VALS)),
+        `(data_at_ Tsh (tarray tuchar 1024) (bufferOut VALS)),
+        `(K_vector KV),
+        `(memory_block dsh (Int.repr 32) (DIGEST A)),
+        `(repr_text a tsh (TEXT A))]).
+       subst Frame. reflexivity.
+     rewrite FR. clear FR Frame.
+     entailer.
+     rewrite HH2 in *. inversion H3; clear H3. subst keylen'. simpl in HH9.
+     assert (KeyLenRangeUnsigned :0 <= key_len a <= Int.max_unsigned).
+       rewrite int_max_unsigned_eq. 
+       destruct HH1 as [KLpos KLsignedBound].
+        rewrite int_max_signed_eq in KLsignedBound; omega.
+     (*rewrite Int.unsigned_repr in *; trivial.*)
+     rewrite (memory_block_array_tuchar' _ (key_len a)); trivial; try omega.
+     entailer. cancel.
+     rewrite <- HH9.
+     rewrite (split_array_at (Zlength (key a))).
+       2: rewrite HH9; omega.
+     cancel.
+     apply array_at_ext'. 
+        intros. unfold tuchars, cVint, ZnthV. simpl.
+          if_tac. omega.
+          destruct (nth_mapVintZ i (key a)) as [? I]; trivial.
+          rewrite I; reflexivity.
+   } 
+   after_call. 
+   (*Warning: Collision between bound variables of name x *)
+   subst WITNESS. normalize. subst retval1.
+ 
+   
+   (**************** memcpy( k_opad, key, key_len ) ******)
+   remember (ksh, Tsh, k_opad VALS, KEY A, key_len a,  
+            force_int oo (ZnthV tuchar (map Vint (map Int.repr (key a))))
+       ) as WITNESS. 
+   forward_call WITNESS.
+   { rewrite HeqWITNESS; clear HeqWITNESS WITNESS.
+     assert (FR: Frame = [
+      `(array_at tuchar Tsh
+        (fun i : Z =>
+         Vint (force_int (ZnthV tuchar (map Vint (map Int.repr (key a))) i))) 0
+        (key_len a) (k_ipad VALS)),
+      `(array_at tuchar Tsh (fun _ : Z => Vint Int.zero) (key_len a) 65 (k_ipad VALS)),
+      `(data_at_ Tsh (tarray tuchar 32) (tk VALS)),
+      `(data_at_ Tsh (tarray tuchar 32) (tk2 VALS)),
+      `(data_at_ Tsh (tarray tuchar 1024) (bufferIn VALS)),
+      `(data_at_ Tsh (tarray tuchar 1024) (bufferOut VALS)),
+      `(K_vector KV),
+      `(repr_text a tsh (TEXT A)),
+      `(memory_block dsh (Int.repr 32) (DIGEST A)),
+      `(array_at tuchar Tsh (fun _ : Z => Vint Int.zero) (key_len a) 65
+          (k_opad VALS))]).
+      subst Frame. reflexivity.
+     rewrite FR. clear FR Frame.
+     entailer.
+     rewrite HH2 in *. inversion H3; clear H3. subst keylen'. 
+     assert (KeyLenRangeUnsigned :0 <= key_len a <= Int.max_unsigned).
+       rewrite int_max_unsigned_eq. 
+       destruct HH1 as [KLpos KLsignedBound].
+        rewrite int_max_signed_eq in KLsignedBound; omega.
+     (*rewrite Int.unsigned_repr in *; trivial.*)
+     apply andp_right. abstract entailer.
+     cancel. 
+     rewrite (split_array_at (key_len a) tuchar Tsh _ 0 65 (k_opad VALS)).
+        2: omega. 
+     rewrite (memory_block_array_tuchar' _ (key_len a)); trivial.
+        2: omega.
+     rewrite HH9.
+     abstract cancel. 
+   } 
+   after_call. 
+   (*Warning: Collision between bound variables of name x *)
+   subst WITNESS. normalize. 
+   subst retval1. 
+
+   (***************for -loop*********************)
+   unfold isPosSigned in HH1.
+   remember ((firstn (Z.to_nat (key_len a)) (key a)) ++ Nlist Z0 (65 - Z.to_nat (key_len a))) as normKey.
+   assert (LN: length normKey = 65%nat).
+     subst. rewrite app_length, firstn_length, length_Nlist.
+     clear - HH9 KLrange GT.
+     rewrite Zlength_correct in HH9; simpl in HH9. 
+     rewrite <- HH9, Nat2Z.id, Min.min_idempotent. omega.
+
+       assert (LK: (length (key a) <= 64)%nat).
+         rewrite <- HH9, Zlength_correct in GT. 
+         apply Z2Nat.inj_le in GT.
+         rewrite Nat2Z.id in GT. apply GT.
+         rewrite <- Zlength_correct. apply initial_world.zlength_nonneg.
+         omega.
+   rewrite (split_array_at 64 tuchar Tsh _ (key_len a) 65); try omega.
+   rewrite (split_array_at 64 tuchar Tsh _ (key_len a) 65); try omega.
+  normalize.
+
+  eapply semax_seq'.
+  frame_SEP 5 0 6 2. 
+  unfold isbyteZ in isByteKey.
+  forward_for_simple_bound 64 (EX i:Z, 
+  (PROP  ()
+   LOCAL  (`(eq (TEXT A)) (eval_id _text); `(eq (KEY A)) (eval_id _key);
+     `(eq KV) (eval_var sha._K256 (tarray tuint 64));
+     `(eq (TEXTLEN A)) (eval_id _text_len);
+     `(eq (KEYLEN A)) (eval_id _key_len); `(eq (DIGEST A)) (eval_id _digest);
+     `(eq (k_ipad VALS)) (eval_var _k_ipad (tarray tuchar 65));
+     `(eq (k_opad VALS)) (eval_var _k_opad (tarray tuchar 65));
+     `(eq (tk VALS)) (eval_var _tk (tarray tuchar 32));
+     `(eq (tk2 VALS)) (eval_var _tk2 (tarray tuchar 32));
+     `(eq (bufferIn VALS)) (eval_var _bufferIn (tarray tuchar 1024));
+     `(eq (bufferOut VALS)) (eval_var _bufferOut (tarray tuchar 1024)))
+   SEP 
+   (
+   `(array_at tuchar Tsh
+       (cVint (force_int oo ZnthV tuchar (map Vint (map Int.repr (map Byte.unsigned (map Byte.repr (HMAC_FUN.mkKey (key a))))))))
+       i 64 (k_opad VALS));
+   `(array_at tuchar Tsh
+       (cVint (force_int oo ZnthV tuchar (map Vint (map Int.repr (map Byte.unsigned (map Byte.repr (HMAC_FUN.mkKey (key a))))))))
+       i 64 (k_ipad VALS));
+   `(array_at tuchar Tsh
+       (cVint (force_int oo ZnthV tuchar (map Vint (map Int.repr (map Byte.unsigned (HMAC_FUN.mkArg (map Byte.repr (HMAC_FUN.mkKey (key a))) Opad))))))
+       0 i (k_opad VALS));
+   `(array_at tuchar Tsh
+       (cVint (force_int oo ZnthV tuchar (map Vint (map Int.repr (map Byte.unsigned (HMAC_FUN.mkArg (map Byte.repr (HMAC_FUN.mkKey (key a))) Ipad))))))
+       0 i (k_ipad VALS))))).
+   
+   { (*precondition implies "invariant"*)
+     rewrite array_at_emp. rewrite array_at_emp. entailer.
+     apply andp_right. unfold array_at. abstract entailer.
+     repeat rewrite (map_map Byte.unsigned). 
+     assert (EQ: forall i : Z, 0 <= i < key_len a ->
+      cVint (force_int oo ZnthV tuchar (map Vint (map Int.repr (key a)))) i =
+      cVint (force_int oo ZnthV tuchar
+        (map Vint
+           (map (fun x : byte => Int.repr (Byte.unsigned x))
+              (map Byte.repr (key a))))) i).
+     { intros; unfold cVint. f_equal; simpl.
+       unfold ZnthV. destruct (zlt i 0); simpl; trivial.
+       assert (I: (0 <= Z.to_nat i < length (key a))%nat).
+         destruct H as [X Y]. 
+         apply Z2Nat.inj_lt in Y.
+         rewrite <- HH9, Zlength_correct, Nat2Z.id in Y. omega. omega. omega.
+       destruct (nth_mapVint (Z.to_nat i) (key a)); trivial.
+       rewrite H12. simpl. rewrite map_map. rewrite map_map.
+       rewrite <- nth_default_eq in H12. unfold nth_default in H12.
+       remember (nth_error (map Vint (map Int.repr (key a))) (Z.to_nat i)) as d. 
+       destruct d; inversion H12. clear H12; subst v. 
+       apply eq_sym in Heqd. destruct (map_nth_error_inv _ _ _  _ Heqd) as [? [? ?]].
+       inv H13; clear Heqd. destruct (map_nth_error_inv _ _ _  _ H12) as [? [? ?]]. subst x0; clear H12.
+       rewrite nth_map' with (d':=Z0). 
+       rewrite <- nth_default_eq. unfold nth_default. rewrite H13.
+       rewrite Byte.unsigned_repr. trivial.
+       rewrite Forall_forall in isByteKey. 
+       apply nth_error_in in H13. apply isByteKey in H13.
+         unfold Byte.max_unsigned, Byte.modulus, Byte.wordsize. simpl. omega.
+       apply I.
+     }
+     rewrite (split_array_at (key_len a) tuchar Tsh _ 0 64); try omega.
+     rewrite (split_array_at (key_len a) tuchar Tsh _ 0 64); try omega.
+     repeat rewrite sepcon_assoc.
+     apply sepcon_derives.
+     apply array_at_ext'. 
+       intros. rewrite EQ; trivial. unfold cVint; simpl. f_equal. f_equal.
+       unfold ZnthV. if_tac. omega. simpl. clear H12.
+       assert (I: (0 <= Z.to_nat i < length (key a))%nat).
+         destruct H as [X Y]. 
+         apply Z2Nat.inj_lt in Y.
+         rewrite <- HH9, Zlength_correct, Nat2Z.id in Y. omega. omega. omega.
+       assert (X: (Z.to_nat i < length (HMAC_FUN.mkKey (key a)))%nat).
+         rewrite HMAC_FUN.mkKey_length. unfold SHA256_BlockSize. omega.
+       repeat rewrite nth_map' with (d':=Int.zero); try repeat rewrite map_length; try omega.
+       f_equal.
+       repeat rewrite nth_map' with (d':=Byte.zero); try repeat rewrite map_length; try omega.
+       f_equal. f_equal.
+         rewrite <- HH9 in H, HeqKLENGTH.
+       repeat rewrite nth_map' with (d':=Z0); try repeat rewrite map_length; try omega.
+       f_equal.
+         erewrite mkKey_left; trivial.
+     apply sepcon_derives.
+     apply array_at_ext'. 
+       clear - KLrange HH9 HeqKLENGTH.
+       intros. unfold cVint; simpl. f_equal. 
+       unfold ZnthV. if_tac. omega. 
+       assert (X: (Z.to_nat i < length (HMAC_FUN.mkKey (key a)))%nat).
+         rewrite HMAC_FUN.mkKey_length. unfold SHA256_BlockSize.
+         destruct H as [X Y].  apply Z2Nat.inj_lt in Y. apply Y. omega. omega.
+       repeat rewrite nth_map' with (d':=Int.zero); try repeat rewrite map_length; try omega.
+       f_equal.
+       repeat rewrite nth_map' with (d':=Byte.zero); try repeat rewrite map_length; try omega.
+       f_equal. f_equal.
+         rewrite <- HH9 in H, HeqKLENGTH.
+       rewrite nth_map' with (d':=Z0); try repeat rewrite map_length; try omega.
+       rewrite mkKey_right; trivial. 
+     apply sepcon_derives. 
+     apply array_at_ext'. 
+       intros. unfold cVint in *. simpl in EQ. rewrite EQ; trivial. simpl. f_equal. f_equal.
+       unfold ZnthV. if_tac. omega. simpl. 
+       assert (I: (0 <= Z.to_nat i < length (key a))%nat).
+         destruct H as [X Y]. 
+         apply Z2Nat.inj_lt in Y.
+         rewrite <- HH9, Zlength_correct, Nat2Z.id in Y. omega. omega. omega.
+       assert (X: (Z.to_nat i < length (HMAC_FUN.mkKey (key a)))%nat).
+         rewrite HMAC_FUN.mkKey_length. unfold SHA256_BlockSize. omega.
+       repeat rewrite nth_map' with (d':=Int.zero); try repeat rewrite map_length; try omega.
+       f_equal.
+       repeat rewrite nth_map' with (d':=Byte.zero); try repeat rewrite map_length; try omega.
+       f_equal. f_equal.
+         rewrite <- HH9 in H, HeqKLENGTH.
+       repeat rewrite nth_map' with (d':=Z0); try repeat rewrite map_length; try omega.
+       f_equal.
+         erewrite mkKey_left; trivial.
+     apply array_at_ext'. 
+       intros. clear EQ. unfold cVint; simpl. f_equal. 
+       unfold ZnthV. if_tac. omega. 
+       assert (X: (Z.to_nat i < length (HMAC_FUN.mkKey (key a)))%nat).
+         rewrite HMAC_FUN.mkKey_length. unfold SHA256_BlockSize.
+         destruct H as [X Y].  apply Z2Nat.inj_lt in Y. apply Y. omega. omega.
+       repeat rewrite nth_map' with (d':=Int.zero); try repeat rewrite map_length; try omega.
+       f_equal.
+       repeat rewrite nth_map' with (d':=Byte.zero); try repeat rewrite map_length; try omega.
+       f_equal. f_equal.
+         rewrite <- HH9 in H, HeqKLENGTH.
+       rewrite nth_map' with (d':=Z0); try repeat rewrite map_length; try omega.
+       rewrite mkKey_right; trivial. 
+   }
+   { (*show that body satisfies "invariant"*)
+     eapply (loopbodyLE Espec); try eassumption.
+   }    
+   { (*show increment*) trivial. (*normalize.*) }
+(*NEW OUT-OF_MEMORY-CRASH emerged here (in the next 5 lines) in svn version 6738 (or a bit before that, since I hadnt updated for a couple of days)*)
+   clear LN HeqnormKey normKey.
+
+   (*normalize. *) unfold update_tycon; simpl.
+   repeat rewrite array_at_emp; simpl. normalize.
+rewrite Zplus_comm in TL1024.
+ 
+(****************** continuation after for-loop **************************)
+ remember (map Byte.unsigned
+                         (HMAC_FUN.mkArg
+                            (map Byte.repr (HMAC_FUN.mkKey (key a))) Ipad))
+     as KIPAD.
+ remember (force_int
+           oo ZnthV tuchar
+                (map Vint (map Int.repr KIPAD))) as IPAD.
+ remember (map Byte.unsigned
+                         (HMAC_FUN.mkArg
+                            (map Byte.repr (HMAC_FUN.mkKey (key a))) Opad))
+     as KOPAD.
+ remember (force_int
+           oo ZnthV tuchar
+                (map Vint (map Int.repr KOPAD))) as OPAD.
+  remember (force_int oo ZnthV tuchar (map Vint (map Int.repr (key a)))) as KKEY. 
+ remember (fun _ : Z => Vint Int.zero) as ZERO.
+
+eapply semax_pre0.
+2: solve [eapply restLE; eassumption].
+abstract solve [entailer; cancel].
+}
+
+Qed.
+
+
+(*Alternative continuation after for-loop *************************
+Require Import HMAC_proofTail.
+eapply semax_pre.
+2: eapply (hmac_LE_tail Espec tsh ksh dsh A a KV text' key' digest' textlen'
+  keylen' perms h0 l Heql Heqh0 VALS HeqKLENGTH GT H0 HH1 HH2 HH3 HH4 TL1024
+  HH5 HH6 HH7 HH8 HH9 TLrange KLrange isByteKey LK); eassumption.
+abstract solve [entailer; cancel].
+}
+Qed.
+*)
+*)
+
+Lemma body_hmac_sha256: semax_body Vprog Gtot 
+      f_hmac_sha256 hmac_spec.
+Proof.
+start_function.
+name text' _text.
+name key' _key.
+name digest' _digest.
+name textlen' _text_len.
+name keylen' _key_len. 
+assert (perms: permissions).
+  unfold permissions, permissions', topshares. 
+  specialize writable_share_top. simpl. intuition.
+simpl_stackframe_of.
+remember {| HMAC_Refined.args := a; 
+            HMAC_Refined.locals := HMAC_Refined.initLocalVals |} as h0.
+remember (tsh, (ksh, dsh)) as argshares.
+apply semax_pre with (P':= EX V: VALUES, ASSN topshares argshares KV initFlags h0 a A A V).
+(*apply semax_pre with (P' := ASSN_EQ topshares argshares initFlags h0 a A A).*)
+  (*unfold interprete, ASSN, ASSN'. *) 
+  unfold (*ASSN_EQ,*) ASSN, ASSN_SuperCanon, f_hmac_sha256.
+  subst argshares. simpl.
+  intros rho. apply exp_right with (x:=ApplyVAR rho).
+  (*apply exp_right with (x:=eval_var sha._K256 (tarray tuint 64) rho).*)
+  unfold ApplyVAR. simpl.
+  unfold prop_args in H; simpl in H.
+  destruct H as [HA1 [HA2 [HA3 [HA4 [HA5 [HA6 HA7]]]]]].
+  unfold sizes, sizes'.
+  unfold repr_locals, repr_local. simpl.
+  abstract solve [entailer; cancel]. 
+unfold (*ASSN_EQ,*) ASSN, ASSN_SuperCanon.
+apply extract_exists_pre; intro VALS.
+(*apply extract_exists_pre; intro KV. *)
+remember (HMAC_Refined.snippet1 h0) as h1.
+specialize (Zgt_cases (key_len a) 64); intros GT.
+normalize.
+remember
+  (if key_len a >? 64 then 
+    {| TEXT := TEXT A;
+       TEXTLEN := TEXTLEN A;
+       KEY := tk VALS; (* take care of assignment key = tk*) 
+       KEYLEN := Vint (Int.repr SHA256_DIGEST_LENGTH); 
+                      (*assignment key_len = SHA256_DIGEST_LENGTH*)
+       DIGEST := DIGEST A |} 
+    else A) as ANEW. 
+remember (args h1) as anew.
+forward_if (ASSN_SuperCanon topshares argshares A ANEW KV
+   {| k_ipad := true;
+                   k_opad := true;
+                   tk:= negb (key_len a >? 64);
+                   tk2:= true;
+                   bufferIn:= true;
+                   bufferOut:= true |} a anew (locals h1) VALS).
+{ (*Then*)
+  make_sequential. simpl. 
+  (*destruct argshares as [tsh [ksh dsh]].*)
+  unfold ASSN_SuperCanon. simpl.
+  unfold repr_key.
+  forward_call (KEY A, key_len a, ksh, tk topshares, key a, tk VALS).
+  { assert (FR: Frame = 
+       [`(data_at_ Tsh (Tarray tuchar 65 noattr) (k_ipad VALS)),
+        `(data_at_ Tsh (Tarray tuchar 65 noattr) (k_opad VALS)), 
+        `(data_at_ Tsh (Tarray tuchar 32 noattr) (tk2 VALS)),
+        `(data_at_ Tsh (Tarray tuchar 1024 noattr) (bufferIn VALS)),
+        `(data_at_ Tsh (Tarray tuchar 1024 noattr) (bufferOut VALS)),
+        `(repr_text a tsh (TEXT A)), `(array_at_ tuchar dsh 0 32 (DIGEST A))]).
+      subst Frame. reflexivity.
+    rewrite FR; clear FR Frame.
+    simpl. intros rho. entailer.
+    unfold repr_locals, repr_key, repr_local. simpl.
+    apply andp_right.  
+      entailer. rewrite H4.
+      destruct H as [[HA1a HA1b] [[HA2a [HA2b TL1024]] [HA3 [HA4 [HA5 [HA6 HA7]]]]]].
+      rewrite <- H4, H5, H6 in *; clear H4 H5 H6.
+      rewrite HA1b, HA2b in *.
+      rewrite Zlength_correct in *.
+      rewrite HA7 in *. simpl. unfold isPosSigned in HA1a.
+      unfold two_power_pos, shift_pos. simpl. 
+      assert (8 * Int.max_signed < 18446744073709551616). 
+        rewrite int_max_signed_eq. omega.
+      entailer. unfold repr_key.
+      apply derives_trans with (Q:=!!(isptr (KEY A) /\ Forall isbyteZ (key a))).
+           entailer. normalize. split; trivial. rewrite int_max_unsigned_eq. rewrite int_max_signed_eq in HA1a. omega.
+    rewrite <- AxiomK. cancel.
+      rewrite memory_block_array_tuchar; try omega.
+      rewrite memory_block_array_tuchar; try omega.
+      rewrite <- (data_at__array_at_ Tsh tuchar 32 noattr(tk VALS)); try omega; trivial.
+   } 
+   after_call.
+   forward.
+   forward. subst ANEW anew. 
+   unfold ASSN_SuperCanon. simpl.
+   intros rho. 
+   entailer.
+   unfold HMAC_Refined.snippet1; simpl.
+   remember (HMAC_Refined.initLocalVals).
+   unfold sem_cast_neutral in H4. simpl in H4. 
+      destruct H as [[HA1a HA1b] [[HA2a [HA2b TL1024]] [HA3 [HA4 [HA5 [HA6 HA7]]]]]].
+     rewrite HA1b in *. unfold force_val, Val.of_bool in H4.
+     unfold both_int in H4. 
+     unfold Int.lt in H4.
+   rewrite Int.signed_repr in H4.
+      Focus 2. rewrite int_min_signed_eq, int_max_signed_eq. omega.
+   rewrite Int.signed_repr in H4.
+      Focus 2. rewrite int_min_signed_eq.
+               unfold isPosSigned in HA1a. omega.
+   destruct (key_len a >? 64).
+   { (*Case key_len a > 64*)
+     clear H4. simpl.
+     unfold repr_locals. 
+     unfold repr_key, repr_text. rewrite Zplus_comm in TL1024. simpl in *.
+     unfold repr_key_len, repr_text_len in *. rewrite Zplus_comm. simpl in *.
+     rewrite HA2b in *; simpl in *. 
+     rewrite Zlength_correct in *. rewrite Zlength_correct. 
+     rewrite length_SHA256'. unfold SHA256_DIGEST_LENGTH. simpl.
+     apply andp_right.
+        unfold isPosSigned. rewrite H3, <- H10.
+        abstract entailer. 
+     rewrite memory_block_array_tuchar; try omega.
+       cancel. rewrite functional_prog.SHA_256'_eq. simpl.
+       rewrite <- HA1b. unfold SEPx. simpl.
+        cancel. entailer. 
+         rewrite <- AxiomK. cancel. }
+   { exfalso.
+     destruct (zlt 64 (key_len a)). omega.
+      discriminate. (* inversion H4.*) }
+  }
+{ (* ELSE*)
+  forward.
+  unfold overridePost, ASSN_SuperCanon; simpl.
+  intros x. unfold repr_locals; simpl. entailer.
+   unfold HMAC_Refined.snippet1; simpl.
+   remember (HMAC_Refined.initLocalVals). 
+   unfold sem_cast_neutral in H2. simpl in H2.
+(*  destruct argshares as [tsh [ksh dsh]]. *)
+     destruct H as [[HH1 HH2] [[HH3 HH4] [HH5 [HH6 [HH7 [HH8 HH9]]]]]].
+     rewrite HH2 in *. unfold force_val, Val.of_bool in H2.
+     unfold both_int in H2. 
+     unfold Int.lt in H2.
+   rewrite <- H6 in *.
+   rewrite Int.signed_repr in H2.
+      Focus 2. rewrite int_min_signed_eq, int_max_signed_eq. omega.
+   rewrite Int.signed_repr in H2.
+      Focus 2. rewrite int_min_signed_eq.
+               unfold isPosSigned in HH1. omega.
+   destruct (key_len a >? 64).
+   { (*Case key_len a > 64*)
+     exfalso. 
+     destruct (zlt 64 (key_len a)). discriminate. (*inversion H2.*) omega. }
+   { unfold repr_key_len, repr_text_len. simpl.
+     rewrite HH9, HH2; simpl.
+     abstract entailer. 
+   }
+}
+(*snippet 2*)
+unfold ASSN_SuperCanon, repr_locals. simpl. normalize.
+
+remember (key_len a >? 64) as KLENGTH.
+destruct KLENGTH.
+{ (* case key_len a > 64 *) admit. }
+
+{ (* case key_len a <= 64 *) 
+  subst ANEW anew. 
+  (*unfold MORE_COMMANDS, POSTCONDITION, abbreviate.*)
+
+  unfold HMAC_Refined.snippet1; simpl.
+  remember (HMAC_Refined.initLocalVals).  
+  assert (Heq: h1 = h0). 
+    subst h1. subst h0. 
+         unfold HMAC_Refined.snippet1; simpl.
+         rewrite <- HeqKLENGTH. reflexivity.
+  clear Heqh1. subst h1. clear H1.
+  subst argshares. clear Heqh0 h0 H0 Heql l.
+  destruct H as [[HH1 HH2] [[HH3 [HH4 TL1024]] [HH5 [HH6 [HH7 [HH8 HH9]]]]]].
+  rewrite HH4 in *.
+  assert (TLrange: 0 <= text_len a <= Int.max_unsigned).
+    clear - HH3. destruct HH3.
+    rewrite int_max_signed_eq in H0. rewrite int_max_unsigned_eq. omega.
+  simpl in HH8. rewrite Int.unsigned_repr in HH8; trivial.
+  assert (KLrange: 0 <= key_len a <= Int.max_unsigned).
+    clear - HH1. destruct HH1.
+    rewrite int_max_signed_eq in H0. rewrite int_max_unsigned_eq. omega.
+  rewrite HH2 in HH9; simpl in HH9.
+    rewrite Int.unsigned_repr in HH9; trivial.
+
+  remember (Tsh, k_ipad VALS, 65, Int.zero) as WITNESS.
+  forward_call (* memset *) WITNESS.
+  { assert (FR: Frame = [
+        `(data_at_ Tsh (tarray tuchar 65) (k_opad VALS)),
+        `(data_at_ Tsh (tarray tuchar 32) (tk VALS)),
+        `(data_at_ Tsh (tarray tuchar 32) (tk2 VALS)),
+        `(data_at_ Tsh (tarray tuchar 1024) (bufferIn VALS)),
+        `(data_at_ Tsh (tarray tuchar 1024) (bufferOut VALS)), 
+        `(K_vector KV),
+        `(repr_key a ksh (KEY A)),
+        `(repr_text a tsh (TEXT A)),
+        `(memory_block dsh (Int.repr 32) (DIGEST A))]).  
+      subst Frame. reflexivity. 
+    rewrite FR. clear FR Frame.
+    unfold repr_locals; simpl. intros rho.
+    entailer.
+    apply andp_right.
+      rewrite <- H5; clear H5. simpl.
+      rewrite (data_at__isptr _ _ (k_ipad VALS)). abstract entailer.
+    assert (SF: Int.repr 65 = Int.repr (sizeof (tarray tuchar 65))) by reflexivity.
+    rewrite SF, align_1_memory_block_data_at_; trivial.
+   }
+   after_call. 
+   (*Warning: Collision between bound variables of name x *)
+   subst WITNESS. normalize. subst retval0.
+
+  forward_call (* memset *) (Tsh, k_opad VALS, 65, Int.zero).
+  { assert (FR: Frame = [
+        `(array_at tuchar Tsh (fun _ : Z => Vint Int.zero) 0 65 (k_ipad VALS)),
+        `(data_at_ Tsh (tarray tuchar 32) (tk VALS)),
+        `(data_at_ Tsh (tarray tuchar 32) (tk2 VALS)),
+        `(data_at_ Tsh (tarray tuchar 1024) (bufferIn VALS)),
+        `(data_at_ Tsh (tarray tuchar 1024) (bufferOut VALS)), 
+        `(K_vector KV),
+        `(repr_key a ksh (KEY A)),
+        `(repr_text a tsh (TEXT A)),
+        `(memory_block dsh (Int.repr 32) (DIGEST A))]).  
+      subst Frame. reflexivity.
+    rewrite FR. clear FR Frame.
+    unfold repr_locals; simpl. intros rho.
+    entailer.
+    apply andp_right.
+      rewrite <- H6; clear H6. simpl.
+      rewrite (data_at__isptr _ _ (k_opad VALS)). abstract entailer.
+    assert (SF: Int.repr 65 = Int.repr (sizeof (tarray tuchar 65))) by reflexivity.
+    rewrite SF, align_1_memory_block_data_at_; trivial. abstract cancel.
+   }
+   after_call. 
+   (*Warning: Collision between bound variables of name x *) 
+   normalize. subst retval0.
+
+   (**************** memcpy( k_ipad, key, key_len ) ******)
+   unfold repr_key, data_block. 
+   eapply semax_pre with (P' :=(PROP (Forall isbyteZ (key a))
+   LOCAL  (
+   `(eq (TEXT A)) (eval_id _text); `(eq (KEY A)) (eval_id _key);
+   `(eq KV) (eval_var sha._K256 (tarray tuint 64));
+   `(eq (TEXTLEN A)) (eval_id _text_len);
+   `(eq (KEYLEN A)) (eval_id _key_len); `(eq (DIGEST A)) (eval_id _digest);
+   `(eq (k_ipad VALS)) (eval_var _k_ipad (tarray tuchar 65));
+   `(eq (k_opad VALS)) (eval_var _k_opad (tarray tuchar 65));
+   `(eq (tk VALS)) (eval_var _tk (tarray tuchar 32));
+   `(eq (tk2 VALS)) (eval_var _tk2 (tarray tuchar 32));
+   `(eq (bufferIn VALS)) (eval_var _bufferIn (tarray tuchar 1024));
+   `(eq (bufferOut VALS)) (eval_var _bufferOut (tarray tuchar 1024)))
+   SEP 
+   (`(array_at tuchar Tsh (fun _ : Z => Vint Int.zero) 0 65 (k_opad VALS));
+   `(array_at tuchar Tsh (fun _ : Z => Vint Int.zero) 0 65 (k_ipad VALS));
+   `(data_at_ Tsh (tarray tuchar 32) (tk VALS));
+   `(data_at_ Tsh (tarray tuchar 32) (tk2 VALS));
+   `(data_at_ Tsh (tarray tuchar 1024) (bufferIn VALS));
+   `(data_at_ Tsh (tarray tuchar 1024) (bufferOut VALS)); `(K_vector KV);
+   `(array_at tuchar ksh (tuchars (map Int.repr (key a))) 0 (Zlength (key a))
+       (KEY A)); `(repr_text a tsh (TEXT A));
+   `(memory_block dsh (Int.repr 32) (DIGEST A))))).
+     abstract entailer. 
+
+   normalize. rename H into isByteKey.
+
+   (* following this recipe doesn't quite work, since some rewrite rule is missing to cleanup
+      the postcondition after after_call
+   eapply semax_seq'.
+   frame_SEP 7 1.*)
+   remember (ksh, Tsh, k_ipad VALS, KEY A, key_len a, 
+            force_int oo (ZnthV tuchar (map Vint (map Int.repr (key a))))
+       ) as WITNESS. 
+   forward_call (* memcopy *) WITNESS.
+   { rewrite HeqWITNESS; clear HeqWITNESS WITNESS.
+     assert (FR: Frame =
+       [`(array_at tuchar Tsh (fun _ : Z => Vint Int.zero) 0 65 (k_opad VALS)),
+        `(array_at tuchar Tsh (fun _ : Z => Vint Int.zero) (Zlength (key a)) 65 (k_ipad VALS)),
+        `(data_at_ Tsh (tarray tuchar 32) (tk VALS)),
+        `(data_at_ Tsh (tarray tuchar 32) (tk2 VALS)),
+        `(data_at_ Tsh (tarray tuchar 1024) (bufferIn VALS)),
+        `(data_at_ Tsh (tarray tuchar 1024) (bufferOut VALS)),
+        `(K_vector KV),
+        `(memory_block dsh (Int.repr 32) (DIGEST A)),
+        `(repr_text a tsh (TEXT A))]).
+       subst Frame. reflexivity.
+     rewrite FR. clear FR Frame.
+     entailer.
+     rewrite HH2 in *. inversion H1; clear H1. subst keylen'. simpl in HH9.
+     assert (KeyLenRangeUnsigned :0 <= key_len a <= Int.max_unsigned).
+       rewrite int_max_unsigned_eq. 
+       destruct HH1 as [KLpos KLsignedBound].
+        rewrite int_max_signed_eq in KLsignedBound; omega.
+     (*rewrite Int.unsigned_repr in *; trivial.*)
+     rewrite (memory_block_array_tuchar' _ (key_len a)); trivial; try omega.
+     entailer. cancel.
+     rewrite <- HH9.
+     rewrite (split_array_at (Zlength (key a))).
+       2: rewrite HH9; omega.
+     cancel.
+     apply array_at_ext'. 
+        intros. unfold tuchars, cVint, ZnthV. simpl.
+          if_tac. omega.
+          destruct (nth_mapVintZ i (key a)) as [? I]; trivial.
+          rewrite I; reflexivity.
+   } 
+   after_call. 
+   (*Warning: Collision between bound variables of name x *)
+   subst WITNESS. normalize. subst retval0.
+ 
+   (**************** memcpy( k_opad, key, key_len ) ******)
+   remember (ksh, Tsh, k_opad VALS, KEY A, key_len a,  
+            force_int oo (ZnthV tuchar (map Vint (map Int.repr (key a))))
+       ) as WITNESS. 
+   forward_call WITNESS.
+   { rewrite HeqWITNESS; clear HeqWITNESS WITNESS.
+     assert (FR: Frame = [
+      `(array_at tuchar Tsh
+        (fun i : Z =>
+         Vint (force_int (ZnthV tuchar (map Vint (map Int.repr (key a))) i))) 0
+        (key_len a) (k_ipad VALS)),
+      `(array_at tuchar Tsh (fun _ : Z => Vint Int.zero) (key_len a) 65 (k_ipad VALS)),
+      `(data_at_ Tsh (tarray tuchar 32) (tk VALS)),
+      `(data_at_ Tsh (tarray tuchar 32) (tk2 VALS)),
+      `(data_at_ Tsh (tarray tuchar 1024) (bufferIn VALS)),
+      `(data_at_ Tsh (tarray tuchar 1024) (bufferOut VALS)),
+      `(K_vector KV),
+      `(repr_text a tsh (TEXT A)),
+      `(memory_block dsh (Int.repr 32) (DIGEST A)),
+      `(array_at tuchar Tsh (fun _ : Z => Vint Int.zero) (key_len a) 65
+          (k_opad VALS))]).
+      subst Frame. reflexivity.
+     rewrite FR. clear FR Frame.
+     entailer.
+     rewrite HH2 in *. inversion H1; clear H1. subst keylen'. 
+     assert (KeyLenRangeUnsigned :0 <= key_len a <= Int.max_unsigned).
+       rewrite int_max_unsigned_eq. 
+       destruct HH1 as [KLpos KLsignedBound].
+        rewrite int_max_signed_eq in KLsignedBound; omega.
+     (*rewrite Int.unsigned_repr in *; trivial.*)
+     apply andp_right. abstract entailer.
+     cancel. 
+     rewrite (split_array_at (key_len a) tuchar Tsh _ 0 65 (k_opad VALS)).
+        2: omega. 
+     rewrite (memory_block_array_tuchar' _ (key_len a)); trivial.
+        2: omega.
+     rewrite HH9.
+     abstract cancel. 
+   } 
+   after_call. 
+   (*Warning: Collision between bound variables of name x *)
+   subst WITNESS. normalize. 
+   subst retval0. 
+
+   (***************for -loop*********************)
+   unfold isPosSigned in HH1.
+   remember ((firstn (Z.to_nat (key_len a)) (key a)) ++ Nlist Z0 (65 - Z.to_nat (key_len a))) as normKey.
+   assert (LN: length normKey = 65%nat).
+     subst. rewrite app_length, firstn_length, length_Nlist.
+     clear - HH9 KLrange GT.
+     rewrite Zlength_correct in HH9; simpl in HH9. 
+     rewrite <- HH9, Nat2Z.id, Min.min_idempotent. omega.
+
+       assert (LK: (length (key a) <= 64)%nat).
+         rewrite <- HH9, Zlength_correct in GT. 
+         apply Z2Nat.inj_le in GT.
+         rewrite Nat2Z.id in GT. apply GT.
+         rewrite <- Zlength_correct. apply initial_world.zlength_nonneg.
+         omega.
+   rewrite (split_array_at 64 tuchar Tsh _ (key_len a) 65); try omega.
+   rewrite (split_array_at 64 tuchar Tsh _ (key_len a) 65); try omega.
+  normalize.
+
+  eapply semax_seq'.
+  frame_SEP 5 0 6 2. 
+  unfold isbyteZ in isByteKey.
+  forward_for_simple_bound 64 (EX i:Z, 
+  (PROP  ()
+   LOCAL  (`(eq (TEXT A)) (eval_id _text); `(eq (KEY A)) (eval_id _key);
+     `(eq KV) (eval_var sha._K256 (tarray tuint 64));
+     `(eq (TEXTLEN A)) (eval_id _text_len);
+     `(eq (KEYLEN A)) (eval_id _key_len); `(eq (DIGEST A)) (eval_id _digest);
+     `(eq (k_ipad VALS)) (eval_var _k_ipad (tarray tuchar 65));
+     `(eq (k_opad VALS)) (eval_var _k_opad (tarray tuchar 65));
+     `(eq (tk VALS)) (eval_var _tk (tarray tuchar 32));
+     `(eq (tk2 VALS)) (eval_var _tk2 (tarray tuchar 32));
+     `(eq (bufferIn VALS)) (eval_var _bufferIn (tarray tuchar 1024));
+     `(eq (bufferOut VALS)) (eval_var _bufferOut (tarray tuchar 1024)))
+   SEP 
+   (
+   `(array_at tuchar Tsh
+       (cVint (force_int oo ZnthV tuchar (map Vint (map Int.repr (map Byte.unsigned (map Byte.repr (HMAC_FUN.mkKey (key a))))))))
+       i 64 (k_opad VALS));
+   `(array_at tuchar Tsh
+       (cVint (force_int oo ZnthV tuchar (map Vint (map Int.repr (map Byte.unsigned (map Byte.repr (HMAC_FUN.mkKey (key a))))))))
+       i 64 (k_ipad VALS));
+   `(array_at tuchar Tsh
+       (cVint (force_int oo ZnthV tuchar (map Vint (map Int.repr (map Byte.unsigned (HMAC_FUN.mkArg (map Byte.repr (HMAC_FUN.mkKey (key a))) Opad))))))
+       0 i (k_opad VALS));
+   `(array_at tuchar Tsh
+       (cVint (force_int oo ZnthV tuchar (map Vint (map Int.repr (map Byte.unsigned (HMAC_FUN.mkArg (map Byte.repr (HMAC_FUN.mkKey (key a))) Ipad))))))
+       0 i (k_ipad VALS))))).
+   
+   { (*precondition implies "invariant"*)
+     rewrite array_at_emp. rewrite array_at_emp. entailer.
+     apply andp_right. unfold array_at. abstract entailer.
+     repeat rewrite (map_map Byte.unsigned). 
+     assert (EQ: forall i : Z, 0 <= i < key_len a ->
+      cVint (force_int oo ZnthV tuchar (map Vint (map Int.repr (key a)))) i =
+      cVint (force_int oo ZnthV tuchar
+        (map Vint
+           (map (fun x : byte => Int.repr (Byte.unsigned x))
+              (map Byte.repr (key a))))) i).
+     { intros; unfold cVint. f_equal; simpl.
+       unfold ZnthV. destruct (zlt i 0); simpl; trivial.
+       assert (I: (0 <= Z.to_nat i < length (key a))%nat).
+         destruct H10 as [X Y]. 
+         apply Z2Nat.inj_lt in Y.
+         rewrite <- HH9, Zlength_correct, Nat2Z.id in Y. omega. omega. omega.
+       destruct (nth_mapVint (Z.to_nat i) (key a)) as [? Hn]; trivial.
+       rewrite Hn. simpl. rewrite map_map. rewrite map_map.
+       rewrite <- nth_default_eq in Hn. unfold nth_default in Hn.
+       remember (nth_error (map Vint (map Int.repr (key a))) (Z.to_nat i)) as d. 
+       destruct d; inversion Hn. clear Hn; subst v. 
+       apply eq_sym in Heqd. destruct (map_nth_error_inv _ _ _  _ Heqd) as [? [? ?]].
+       inv H12; clear Heqd. destruct (map_nth_error_inv _ _ _  _ H11) as [? [? ?]]. 
+       subst x0; clear H11.
+       rewrite nth_map' with (d':=Z0). 
+       rewrite <- nth_default_eq. unfold nth_default. rewrite H12.
+       rewrite Byte.unsigned_repr. trivial.
+       rewrite Forall_forall in isByteKey. 
+       apply nth_error_in in H12. apply isByteKey in H12.
+         unfold Byte.max_unsigned, Byte.modulus, Byte.wordsize. simpl. omega.
+       apply I.
+     }
+     rewrite (split_array_at (key_len a) tuchar Tsh _ 0 64); try omega.
+     rewrite (split_array_at (key_len a) tuchar Tsh _ 0 64); try omega.
+     repeat rewrite sepcon_assoc.
+     apply sepcon_derives.
+     apply array_at_ext'. 
+       intros. rewrite EQ; trivial. unfold cVint; simpl. f_equal. f_equal.
+       unfold ZnthV. if_tac. omega. simpl. clear H11.
+       assert (I: (0 <= Z.to_nat i < length (key a))%nat).
+         destruct H10 as [X Y]. 
+         apply Z2Nat.inj_lt in Y.
+         rewrite <- HH9, Zlength_correct, Nat2Z.id in Y. omega. omega. omega.
+       assert (X: (Z.to_nat i < length (HMAC_FUN.mkKey (key a)))%nat).
+         rewrite HMAC_FUN.mkKey_length. unfold SHA256_BlockSize. omega.
+       repeat rewrite nth_map' with (d':=Int.zero); try repeat rewrite map_length; try omega.
+       f_equal.
+       repeat rewrite nth_map' with (d':=Byte.zero); try repeat rewrite map_length; try omega.
+       f_equal. f_equal.
+         rewrite <- HH9 in H10, HeqKLENGTH.
+       repeat rewrite nth_map' with (d':=Z0); try repeat rewrite map_length; try omega.
+       f_equal.
+         erewrite mkKey_left; trivial.
+     apply sepcon_derives.
+     apply array_at_ext'. 
+       clear - KLrange HH9 HeqKLENGTH.
+       intros. unfold cVint; simpl. f_equal. 
+       unfold ZnthV. if_tac. omega. 
+       assert (X: (Z.to_nat i < length (HMAC_FUN.mkKey (key a)))%nat).
+         rewrite HMAC_FUN.mkKey_length. unfold SHA256_BlockSize.
+         destruct H as [X Y].  apply Z2Nat.inj_lt in Y. apply Y. omega. omega.
+       repeat rewrite nth_map' with (d':=Int.zero); try repeat rewrite map_length; try omega.
+       f_equal.
+       repeat rewrite nth_map' with (d':=Byte.zero); try repeat rewrite map_length; try omega.
+       f_equal. f_equal.
+         rewrite <- HH9 in H, HeqKLENGTH.
+       rewrite nth_map' with (d':=Z0); try repeat rewrite map_length; try omega.
+       rewrite mkKey_right; trivial. 
+     apply sepcon_derives. 
+     apply array_at_ext'. 
+       intros. unfold cVint in *. simpl in EQ. rewrite EQ; trivial. simpl. f_equal. f_equal.
+       unfold ZnthV. if_tac. omega. simpl. 
+       assert (I: (0 <= Z.to_nat i < length (key a))%nat).
+         destruct H10 as [X Y]. 
+         apply Z2Nat.inj_lt in Y.
+         rewrite <- HH9, Zlength_correct, Nat2Z.id in Y. omega. omega. omega.
+       assert (X: (Z.to_nat i < length (HMAC_FUN.mkKey (key a)))%nat).
+         rewrite HMAC_FUN.mkKey_length. unfold SHA256_BlockSize. omega.
+       repeat rewrite nth_map' with (d':=Int.zero); try repeat rewrite map_length; try omega.
+       f_equal.
+       repeat rewrite nth_map' with (d':=Byte.zero); try repeat rewrite map_length; try omega.
+       f_equal. f_equal.
+         rewrite <- HH9 in H10, HeqKLENGTH.
+       repeat rewrite nth_map' with (d':=Z0); try repeat rewrite map_length; try omega.
+       f_equal.
+         erewrite mkKey_left; trivial.
+     apply array_at_ext'. 
+       intros. clear EQ. unfold cVint; simpl. f_equal. 
+       unfold ZnthV. if_tac. omega. 
+       assert (X: (Z.to_nat i < length (HMAC_FUN.mkKey (key a)))%nat).
+         rewrite HMAC_FUN.mkKey_length. unfold SHA256_BlockSize.
+         destruct H10 as [X Y].  apply Z2Nat.inj_lt in Y. apply Y. omega. omega.
+       repeat rewrite nth_map' with (d':=Int.zero); try repeat rewrite map_length; try omega.
+       f_equal.
+       repeat rewrite nth_map' with (d':=Byte.zero); try repeat rewrite map_length; try omega.
+       f_equal. f_equal.
+         rewrite <- HH9 in H10, HeqKLENGTH.
+       rewrite nth_map' with (d':=Z0); try repeat rewrite map_length; try omega.
+       rewrite mkKey_right; trivial. 
+   }
+   { (*show that body satisfies "invariant"*)
+     eapply (loopbodyLE Espec); try eassumption.
+   }    
+   { (*show increment*) trivial. (*normalize.*) }
+
+   clear LN HeqnormKey normKey.
+   (*normalize. *) unfold update_tycon; simpl.
+   repeat rewrite array_at_emp; simpl. normalize.
+
+rewrite Zplus_comm in TL1024.
+ 
+(****************** continuation after for-loop **************************)
+ remember (map Byte.unsigned
+                         (HMAC_FUN.mkArg
+                            (map Byte.repr (HMAC_FUN.mkKey (key a))) Ipad))
+     as KIPAD.
+ remember (force_int
+           oo ZnthV tuchar
+                (map Vint (map Int.repr KIPAD))) as IPAD.
+ remember (map Byte.unsigned
+                         (HMAC_FUN.mkArg
+                            (map Byte.repr (HMAC_FUN.mkKey (key a))) Opad))
+     as KOPAD.
+ remember (force_int
+           oo ZnthV tuchar
+                (map Vint (map Int.repr KOPAD))) as OPAD.
+  remember (force_int oo ZnthV tuchar (map Vint (map Int.repr (key a)))) as KKEY. 
+ remember (fun _ : Z => Vint Int.zero) as ZERO.
+
+eapply semax_pre0.
+Focus 2. eapply restLE; try eassumption. reflexivity. reflexivity.
+abstract solve [entailer; cancel].
+}
+
+Qed.
+
+
+(*Alternative continuation after for-loop *************************
+Require Import HMAC_proofTail.
+eapply semax_pre.
+2: eapply (hmac_LE_tail Espec tsh ksh dsh A a KV text' key' digest' textlen'
+  keylen' perms h0 l Heql Heqh0 VALS HeqKLENGTH GT H0 HH1 HH2 HH3 HH4 TL1024
+  HH5 HH6 HH7 HH8 HH9 TLrange KLrange isByteKey LK); eassumption.
+abstract solve [entailer; cancel].
+}
+Qed.
+*)
